Compiler: (WIP) Top-level strategy

Clap/Compiler/Traverse.lean
@@ -6,6 +6,7 @@ import Lean.Meta.Tactic.Cbv.Main
 
 import Clap.Lang
 import Clap.Spec
+import Clap.Compiler.Constraints
 import Clap.Compiler.Simp
 import Clap.Compiler.Vectors
 import Clap.Compiler.Wheels
@@ -14,27 +15,11 @@ namespace Clap.Compiler
 
 open Lean Meta Qq Elab
 
-instance {m} [Monad m] : Union (m Sym.Simp.Methods) where
-  union a b := do return (←a) ∪ (←b)
+instance {m} [Monad m] : AndThen (m Sym.Simp.Methods) where
+  andThen a b := do return (←a) >> (←b ())
 
-theorem _root_.List.drop_toArray {α} {l : List α} {i} :
-  l.toArray.drop i = (l.drop i).toArray := by
-  simp only [
-    Array.drop_eq_extract, List.size_toArray, List.extract_toArray,
-    List.extract_eq_take_drop, Array.mk.injEq
-  ]
-  rw [←List.extract_eq_take_drop, List.drop_eq_extract]
-
-/--
-YEEEEEHAAAAAAAAW, you rootin' tootin' cowboy.
--/
-def cowboyCast (e : Expr) (yourDeepestDesire : ℕ) : Sym.SymM Expr := do
-  let t ← Sym.inferType e
-  let_expr Vector t sz := t | throwError m!"Not a true cowboy."
-  let proof ← mkEq t (←mkAppM ``Vector #[t, mkNatLit yourDeepestDesire]) -- TODO: Nuke mapM
-  let e' ← e.rewriteType (←mkSorry proof false)
-  logInfo m!"Cowboy cast:\n{e}\n==>\n{e'}"
-  return e'
+@[inherit_doc Simp.wrapped]
+abbrev singlePass := Simp.wrapped
 
 namespace SymSets
 
@@ -58,23 +43,106 @@ def getSimproc (name : Name) : MetaM Sym.Simp.Simproc := do
 
 def orElse (names : Array Name) : MetaM Sym.Simp.Simproc := do
   let simprocs ← names.mapM getSimproc
-  return simprocs.foldl (· <|> ·) (fun _ ↦ return .rfl) -- I hope this is the `.continue`...
+  return simprocs.foldl (· <|> ·) (fun _ ↦ return .rfl)
 
 def andThen (names : Array Name) : MetaM Sym.Simp.Simproc := do
   let simprocs ← names.mapM getSimproc
-  return simprocs.foldl (· >> ·) (fun _ ↦ return .rfl) -- I hope this is the `.continue`...
+  return simprocs.foldl (· >> ·) (fun _ ↦ return .rfl)
+
+/--
+A simproc with logging enabled.
+-/
+def withLog (name : String) (f : Simproc) : Simproc :=
+  fun e ↦ do
+    let (res, time) ← Dbg.timeS (f e)
+    match res with
+      | .rfl .. =>
+        recordSkippedRuleDbg name time
+        return res
+      | .step e' .. =>
+        recordRuleDbg name time
+        trace[Clap.Compile.dbg] m!"\n[{name}]\n{e}\n==>\n{e'}"
+        return res
+
+/--
+A simproc of sequenced simprocs with logging enabled.
+-/
+def andThenWithLog (names : Array Name) : MetaM Sym.Simp.Simproc := do
+  let simprocs ← names.mapM getSimproc
+  return (simprocs.zip names).foldl (init := fun _ ↦ return .rfl) fun acc (proc, name) ↦
+    acc >> withLog name.lastComponent!.toString proc
+
+/--
+A variation on `Lean.Meta.Sym.Simp.Theorems.rewrite` that composes with a logging proc.
+-/
+def _root_.Lean.Meta.Sym.Simp.Theorems.rewriteWithLog
+  (thms : Theorems) (d : Discharger := dischargeNone) : Simproc := fun e => do
+  let mut anyCD := false
+  for (thm, numExtra) in thms.getMatchWithExtra e do
+    let rw := withLog thm.declName.get!.lastComponent!.toString (thm.rewrite (d := d))
+    let result ←
+      if numExtra == 0
+      then rw e
+      else simpOverApplied e numExtra rw
+    anyCD := anyCD || result.isContextDependent
+    if !result.isRfl then
+      return if anyCD && !result.isContextDependent then result.withContextDependent else result
+  return mkRflResultCD anyCD
+
+def mkSimprocForWithLog (declNames : Array Name) (d : Discharger := dischargeNone) : MetaM Simproc := do
+  let mut thms : Theorems := {}
+  for declName in declNames do
+    thms := thms.insert (← mkTheoremFromDecl declName)
+  return thms.rewrite d
 
 def mkPostMethods (declNames : Array Name)
-                  (d : Discharger := Sym.Simp.dischargeSimpSelf) : MetaM Methods := do
+                  (d : Discharger := Sym.Simp.dischargeNone) : MetaM Methods := do
   let (procs, thms) ← declNames.toList.partitionM (liftM ∘ isSimproc)
-  let procs ← andThen procs.toArray
-  return { post := (←mkSimprocFor thms.toArray d) >> procs }
+  let procs ← andThenWithLog procs.toArray
+
+  let totalName := declNames.foldl (λ acc name => name.toString ++ acc) ""
+  let proc := withLog totalName ((←mkSimprocFor thms.toArray d) >> procs)
+
+  return { post := proc }
+
+/--
+I thought this would sigle-pass, but apparently not.
+-/
+def mkPostMethodsSinglePass (declNames : Array Name)
+                            (d : Discharger := Sym.Simp.dischargeSimpSelf) : MetaM Methods := do
+  let (procs, thms) ← declNames.toList.partitionM (liftM ∘ isSimproc)
+  let procs ← orElse procs.toArray
+  return { post := procs >> (←mkSimprocFor thms.toArray d) }
 
 def mkPreMethods (declNames : Array Name)
-                 (d : Discharger := Sym.Simp.dischargeSimpSelf) : MetaM Methods := do
+                 (d : Discharger := Sym.Simp.dischargeNone) : MetaM Methods := do
   let (procs, thms) ← declNames.toList.partitionM (liftM ∘ isSimproc)
+  let totalName := declNames.foldl (λ acc name => name.toString ++ acc) ""
   let procs ← andThen procs.toArray
-  return { pre := (←mkSimprocFor thms.toArray d) >> procs }
+  let proc := withLog totalName (procs >> (←mkSimprocFor thms.toArray d))
+  return { pre := proc }
+
+inductive PrePost where | Pre | Post
+  deriving DecidableEq, Repr
+
+instance : Inhabited PrePost := ⟨.Post⟩
+
+def mkMethods (components : Array (Name × PrePost))
+              (d : Discharger := Sym.Simp.dischargeSimpSelf) : MetaM Methods := do
+  let (procs, thms) ← components.toList.partitionM fun (name, _) ↦ isSimproc name
+  let (preProcs, postProcs) := partitionPrePost procs
+  let (preThms, postThms) := partitionPrePost thms
+  let preProcs ← andThenWithLog preProcs.toArray
+  let preThms ← mkSimprocForWithLog preThms.toArray d
+  let postProcs ← andThenWithLog postProcs.toArray
+  let postThms ← mkSimprocForWithLog postThms.toArray d
+
+  let pre := preProcs >> preThms
+  let post := postProcs >> postThms
+  return { pre := pre, post := post }
+
+  where partitionPrePost (arg : List (Name × PrePost)) :=
+    (arg.partition fun (_, prePost) ↦ prePost matches .Pre).map (·.map Prod.fst) (·.map Prod.fst)
 
 namespace Monad
 
@@ -103,13 +171,34 @@ private def zetaReduce : Simproc := fun e ↦ do
     m!"\n{e}\n==>\n{new}"
   return .step new (←Sym.mkEqRefl new)
 
+def getApplicationChain (e: Expr) (depth: ℕ): Option (Expr × List Expr) := do
+  if depth = 0 then .none
+  let .app function arg := e | .none
+  let .some (inner_function, args) := getApplicationChain function (depth - 1) | .some (function, [arg])
+  return (inner_function, arg::args)
+
 /--
 This is more or less `Lean.Meta.Tactic.Cbv.betaReduce`, which seems to not be exported.
 -/
 def betaReduce : Simproc := fun e ↦ do
-  let new := e.headBeta
-  let new ← Sym.share new
-  return .step new (←Sym.mkEqRefl new)
+  -- let (function@(.lam ..), args@⟨(.cons _ _)⟩) := e.withApp (·, ·) | return .rfl
+  -- let Expr.app function arg := e | return .rfl
+  -- let (Expr.lam _ _ _ _) := function | return .rfl
+  let .some (function, args) := getApplicationChain e 2 | return .rfl
+  -- Dbg.timeSince timeα "getApp[2]"
+
+  -- let timeα ← IO.monoMsNow
+  -- let .some (function, args) := getApplicationChain e 1 | return .rfl
+  -- Dbg.timeSince timeα "getApp[1]"
+
+  -- logWarning m!"function: {function}\nargs: {args}\nfunction: {function'}\nargs': {args'}"
+  let .lam _ _ _ _ := function | return .rfl
+  let args := args.toArray
+  let e' ← Sym.shareCommonInc <| function.betaRev args
+
+  trace[Clap.Compile.simp.proc.beta]
+    m!"\n{e}\n==>\n{e'}\nharr:{args.size}"
+  return .step e' (←Sym.mkEqRefl e')
 
 def zeta : MetaM Methods := do
   return {
@@ -117,14 +206,38 @@ def zeta : MetaM Methods := do
   }
 
 def beta : MetaM Methods := do
-  return {
-    pre := betaReduce
-  }
+  mkPreMethods #[
+    `Clap.Compiler.SymSets.General.betaReduce
+  ]
+  ∪
+  mkPostMethods #[
+    `Clap.Compiler.SymSets.General.betaReduce
+  ]
 
 def control : MetaM Methods := do
   return {
     pre := simpControl
   }
+
+def compilerSet_bind_eq_bind : MetaM Sym.Simp.Methods :=
+  mkPostMethods #[
+    ``Option.bind_eq_bind
+  ]
+
+def compilerSet_bind_assoc : MetaM Sym.Simp.Methods :=
+  mkPostMethods #[
+    ``Option.bind_assoc, ``bind_assoc
+  ]
+
+def compilerSet_bind_pure : MetaM Sym.Simp.Methods :=
+  mkPostMethods #[
+    ``Option.bind_some, ``bind_pure, ``pure_bind
+  ]
+
+def compilerSet_bind_some : MetaM Sym.Simp.Methods :=
+  mkPostMethods #[
+    ``Option.bind_some
+  ]
 
 def compilerSet_whatever : MetaM Sym.Simp.Methods :=
   mkPostMethods #[
@@ -132,6 +245,11 @@ def compilerSet_whatever : MetaM Sym.Simp.Methods :=
     ``Option.pure_def,
     ``Option.bind_eq_bind, ``Option.bind_fun_some, ``Option.bind_some, ``bind_pure, ``pure_bind,
     ``Option.map_eq_map, ``Option.map_some, ``Option.pure_apply
+  ]
+
+def optionPureApply : MetaM Sym.Simp.Methods :=
+  mkPostMethods #[
+    ``Option.pure_apply
   ]
 
 def compilerSet_old : MetaM Sym.Simp.Methods :=
@@ -159,84 +277,144 @@ def compilerSet : MetaM Sym.Simp.Methods :=
     ``Option.pure_def, ``Option.bind_some, ``Option.bind_eq_bind
   ]
 
-def heh : Sym.Simp.Simproc := fun e ↦ do
-  -- logInfo m!"heh: {e}"
-  -- let time ← IO.monoMsNow
+-- `fun x ↦ (x, fun x ↦ x)`
+
+/--
+TODO: Account for `PUnit` and such.
+-/
+def isOptionUnit (e : Expr) : Bool := Id.run do
+  let_expr Option x := e | return false
+  return x.isConstOf ``Unit
+
+-- vec ==> #v[vec[0], vec[1]][0] : GetElem (1 + 1)
+-- Vector.mk 2 ... |>.getElem (1 + 1)
+
+def monad : Sym.Simp.Simproc := fun e ↦ do
   match_expr e with
-  | Option.bind _ _ a f => 
-    let_expr Option.some _ a := a | return .rfl
-    let e' ← Sym.shareCommonInc (f.beta #[a])
-    return .step e' (←Sym.mkEqRefl e') -- `Option.bind_some`
-
-    -- let thm ← mkTheoremFromDecl ``Option.bind_some
-    -- let res ← thm.rewrite e
-    -- -- Dbg.timeSince time "heh: "
-    -- -- (res.getResultExpr e).checkMaxShared
-    -- return res
-
-  | Pure.pure m _ t x =>
-    if !m.isConstOf ``Option then return .rfl
-    -- let thm ← mkTheoremFromDecl ``Option.pure_apply -- TODO: Probably cache this
-    -- let res ← thm.rewrite e
-    -- (res.getResultExpr e).checkMaxShared
-    -- Dbg.timeSince time "heh: "
-    -- return res
-    logInfo m!"m: {m}\nt: {t}\nx: {x}"
-    let e' ← Sym.shareCommon (mkApp2 (.const ``Option.some [←Sym.getLevelInType t]) t x)
+  | Bind.bind _ _ α β x f =>
+    let u ← Sym.getLevelInType α
+    let v ← Sym.getLevelInType β
+    let e' ← shareCommonInc <| mkApp4 (.const ``Option.bind [u, v]) α β x f
+    trace[Clap.Compile.simp.proc.monad.bind_eq_bind]
+      m!"\n{e}\n==>\n{e'}"
     return .step e' (←Sym.mkEqRefl e')
-  | _ => return .rfl
+  | Pure.pure _ _ α x =>
+    let u ← Sym.getLevelInType α
+    let e' ← shareCommonInc <| mkApp2 (.const ``Option.some [u]) α x
+    trace[Clap.Compile.simp.proc.monad.pure_apply]
+      m!"\n{e}\n==>\n{e'}"
+    return .step e' (←Sym.mkEqRefl e')
+  | Option.bind α γ x g =>
+    match_expr x with
+    -- | Option.bind α β x f =>
+    --   -- let time ← IO.monoMsNow
+    --   let subtree := (←Sym.simp f).getResultExpr f
+    --   trace[Clap.Compile.simp.proc.monad.bind_assoc]
+    --     m!"Subtree.\n{f}\n==>\n{subtree}"
+    --   let u ← Sym.getLevelInType α
+    --   let v ← Sym.getLevelInType β
+    --   let w ← Sym.getLevelInType γ
+    --   -- `f : α → m β | g : β → m γ | x : m α`
+    --   let bind ← shareCommonInc <|
+    --     mkApp4 (.const ``Option.bind [v, w]) β γ (←shareCommonInc (f.beta #[.bvar 0])) g
+    --   let cont := Expr.lam `_assoc α bind .default
+    --   let e' ← shareCommonInc <| mkApp4 (.const ``Option.bind [u, w]) α γ x cont
+    --   trace[Clap.Compile.simp.proc.monad.bind_assoc]
+    --     m!"\n{e}\n==>\n{e'}"
+    --   -- Dbg.timeSince time "bind_assoc took:"
+    --   return .step e' (←mkSorry (←mkEq e e') false)
+    | Option.some _ x =>
+      let e' ← shareCommonInc (g.beta #[x])
+      trace[Clap.Compile.simp.proc.monad.bind_some]
+        m!"\n{e}\n==>\n{e'}"
+      return .step e' (←Sym.mkEqRefl e')
+    | _ => return .rfl
+    -- | _ =>
+    --   -- addConstraint q(Nat)
+    --   -- logInfo m!"res: {←getConstraints}" -- x >>= f
+    --   let x' := (←Sym.simp x (←read).toMethods).getResultExpr x
+    --   if isSameExpr x x' then
+    --     trace[Clap.Compile.simp.proc.monad.top_level]
+    --       m!"{checkEmoji} {x'}"
+    --     return .rfl
+    --   else
+    --     trace[Clap.Compile.simp.proc.monad.top_level]
+    --       m!"\n{x}\n==>ₗ\n{x'}"
+    --   let g' := (←Sym.simp g).getResultExpr g
+    --   trace[Clap.Compile.simp.proc.monad.top_level]
+    --     m!"\n{g}\n==>ᵣ\n{g'}"
+    --   let e' ← shareCommonInc <|
+    --     mkApp4 (.const ``Option.bind [←Sym.getLevelInType α, ←Sym.getLevelInType γ]) α γ x' g'
+    --   trace[Clap.Compile.simp.proc.monad.top_level]
+    --     m!"\n{e}\n==>\n{e'}"
+    --   return .step e' (←mkSorry (←mkEq e e') false)
+  | _ =>
+    return .rfl
 
-def compilerSetAlt2 : MetaM Sym.Simp.Methods :=
-  mkPostMethods (d := Sym.Simp.dischargeNone) #[
-    -- ``heh
-    -- ``Option.bind_some,
-    ``Option.pure_apply
+-- def _root_.Lean.Expr.matchBindsE (e : Expr) : Option (Expr × Expr) :=
+--   match_expr e with
+--   | Bind.bind _ _ _ _ a f => .some (a, f)
+--   | Option.bind   _ _ a f => .some (a, f)
+--   | _                     => .none
+
+-- def _root_.Lean.Expr.matchBindsEInfo (e : Expr) : Option (List Level × Array Expr) :=
+--   match_expr e with
+--   | Bind.bind _ _ α β a f => .some (e.getAppFn.constLevels!, #[α, β, a, f])
+--   | Option.bind   α β a f => .some (e.getAppFn.constLevels!, #[α, β, a, f])
+--   | _                     => .none
+
+def bind_eq_bind_sym {α} {β} := (Option.bind_eq_bind (α := α) (β := β)).symm
+
+def compilerBindEqBind : MetaM Sym.Simp.Methods :=
+  mkPostMethods #[
+    ``bind_eq_bind_sym
   ]
 
--- /--
--- TODO: Highly experimental.
--- -/
--- def castGround : Simproc := fun e ↦ do
---   let t ← Sym.inferType e
---   let normalForm ← simpWithGround t
---   if isSameExpr t (normalForm.getResultExpr t)
---   then return .rfl
---   -- TODO: Probably not the best idea.
---   -- We are using `.mp` to detect that a cast has already ocurred, which might not be so smart.
---   if e.isAppOf ``Eq.mp then return .rfl
---   let proof : SymM Expr :=
---     match normalForm with
---     | .rfl .. => Sym.mkEqRefl t
---     | .step _ prf .. => return prf
---   let univ ← Sym.getLevel (normalForm.getResultExpr t)
---   let e' := mkApp4 (.const ``Eq.mp [univ]) t (normalForm.getResultExpr t) (←proof) e
---   trace[Clap.Compile.simp.proc.preprocess]
---     m!"\n{e}\n==>\n{e'}\n\n{t}\n=t=>\n{(normalForm.getResultExpr t)}"
---   return .step e' (←mkSorry (←mkEq e e') false)
+-- def monadBindAssoc : Sym.Simp.Simproc := fun e ↦ do
+--   match e.matchBindsEInfo with
+--   | .some (_, #[_, γ, x, g]) =>
+--     match x.matchBindsEInfo with
+--     | .some (_, #[α, β, x, f]) =>
+--       -- let subtree := (←Sym.simp f).getResultExpr f
+--       -- trace[Clap.Compile.simp.proc.monad.bind_assoc]
+--       --   m!"Subtree.\n{f}\n==>\n{subtree}"
+--       let u ← Sym.getLevelInType α
+--       let v ← Sym.getLevelInType β
+--       let w ← Sym.getLevelInType γ
+--       -- `f : α → m β | g : β → m γ | x : m α`
+--       let bind ← shareCommonInc <|
+--         mkApp4 (.const ``Option.bind [v, w]) β γ (←shareCommonInc (f.beta #[.bvar 0])) g
+--       let cont := Expr.lam `_assoc α bind .default
+--       let e' ← shareCommonInc <| mkApp4 (.const ``Option.bind [u, w]) α γ x cont
+--       inDebugOnly (do
+--         recordDbgHisto x
+--       )
+--       trace[Clap.Compile.proc.monad.bind_assoc]
+--         m!"INLINED: {x}\n{(←Sym.simp e (←compilerBindEqBind)).getResultExpr e}\n==>\n{(←Sym.simp e' (←compilerBindEqBind)).getResultExpr e'}"
+--       return .step e' (←mkSorry (←mkEq e e') false)
+--     | _ =>
+--       return .rfl
+--   | _ => return .rfl
 
--- def cast : MetaM Methods :=
---   mkPostMethods #[
---     ``castGround
+def monadBindAssocSimple : MetaM Sym.Simp.Methods :=
+  mkPreMethods #[
+    ``Option.bind_assoc
+  ]
 
---     -- ``appendDbg
---   ]
+def monads : MetaM Sym.Simp.Methods :=
+  mkPreMethods #[
+    ``monad,
+  ]
 
--- private def seemsTotallySafeInDTT : Simproc := fun e ↦ do
---   let_expr Vector _ n := ←Sym.inferType e | return .rfl
---   let groundSize := (←Sym.simp n (←ground)).getResultExpr n
---   if isSameExpr n groundSize then return .rfl
---   match groundSize.nat? with
---   | .none => throwError m!"{groundSize} is not ground.\nTODO: Maybe this is ok."
---   | .some groundSize =>
---     let cowboyCast e _
---     trace[Clap.Compile.simp.proc.seemsTotallySafeInDTT]
---       m!"{}"
---     return .rfl
---   -- let e' ← Sym.Simp.evalGround {} e
---   -- unless isSameExpr e (e'.getResultExpr e) do
---   --   trace[Clap.Compile.simp.proc.evalGround]
---   --     m!"\n{e}\n==>\n{e'.getResultExpr e}"
---   -- return e'
+def compilerAssoc : MetaM Sym.Simp.Methods :=
+  mkPreMethods #[
+    ``monadBindAssoc
+  ]
+
+def compilerAssocPost : MetaM Sym.Simp.Methods :=
+  mkPostMethods #[
+    ``monadBindAssoc
+  ]
 
 end General
 
@@ -292,175 +470,468 @@ def vectorElemsOfMk (e : Expr) : Option (Array Expr × Expr × Expr) := do
   return (←arrayElemsOfExpr arr, t, sz)
 
 /--
-We're already doing O(n) work in `listElemsOfExpr` anyway, maybe yield the goodies as well.
+TODO: Maybe generalise this to `GetElem` supporting collections, but it's not relevant
+for the current project.
 -/
-partial def listElemsOfExpr' (e : Expr) (res : Array Expr × ℕ := (#[], 0)) :
-                             Option (Array Expr × Expr × ℕ) :=
-  match_expr e with
-  | List.cons _ hd tl => listElemsOfExpr' tl (res.1.push hd, res.2.succ)
-  | List.nil  α       => .some (res.1, α, res.2)
-  | _                 => .none
+inductive CollectionKind where | Vector | Array | List
+  deriving Repr
 
-def arrayElemsOfExpr' (e : Expr) : Option (Array Expr × Expr × ℕ) := do
-  let_expr Array.mk _ l := e | .none
-  listElemsOfExpr' l
+structure CollectionType where
+  private _mk ::
+  t  : Expr
+  k  : CollectionKind
+  sz : Option Expr
+  deriving Repr
+
+def CollectionType.cast (c : CollectionType) (t : CollectionKind) : Option CollectionType :=
+  match t with
+  | .Vector => if c.sz.isNone then .none else go c t
+  | _       => go c t
+  where go (c : CollectionType) (k : CollectionKind) : CollectionType := {c with k := k}
+
+def CollectionType.setSize (c : CollectionType) (sz : Expr) : CollectionType :=
+  {c with sz := .some sz}
+
+def CollectionType.mkList (elem : Expr) := CollectionType._mk elem .List .none
+
+def CollectionType.mkArray (elem : Expr) := CollectionType.mkList elem |>.cast .Array
+
+def CollectionType.mkVec (elem : Expr) (sz : Expr) :=
+  CollectionType.mkList elem |>.setSize sz |>.cast .Vector
+
+structure Collection where
+  type     : CollectionType
+  listExpr : Expr
+  deriving Repr
+
+def Collection.setSize (coll : Collection) (sz : Expr) : Collection :=
+  {coll with type := coll.type.setSize sz}
 
 /--
-Currently separate from the `vectorElemsOfMk` chain.
+We're already doing O(n) work in `listElemsOfExpr` anyway, maybe yield the goodies as well.
 -/
-def elemsOfColl (e : Expr) : Option (Array Expr × Expr × Expr) :=
+partial def elemsOfListExpr (e : Expr) (elems : Array Expr := #[]) (sz : ℕ := 0) : Array Expr × ℕ :=
   match_expr e with
-  | Vector.mk _ _ _ _ => vectorElemsOfMk e
-  | Array.mk _ _      => spoon <$> arrayElemsOfExpr' e
-  | _                 => spoon <$> listElemsOfExpr' e
-  where spoon := fun (arr, t, sz) ↦ (arr, t, toExpr sz)
+  | List.cons _ hd tl => elemsOfListExpr tl (elems.push hd) sz.succ
+  | _                 => (elems, sz) -- `List.nil` and `_`
+
+def Collection.elems (c : Collection) : Array Expr × Collection :=
+  let (elems, sz) := elemsOfListExpr c.listExpr
+  ⟨elems, c.setSize (toExpr sz)⟩
+
+def Collection.toExpr (c : Collection) : Sym.Simp.SimpM Expr := do
+  match c.type.k with
+  | .List => return c.listExpr
+  | .Array => shareCommonInc <| mkAppN (.const ``Array.mk [←Sym.getLevelInType c.type.t])
+                                       #[c.type.t, c.listExpr]
+  | .Vector => shareCommonInc (←mkVecLit c.type.t c.listExpr (←c.type.sz.getDM (unreachable!)))
+
+def Collection.ofExpr (e : Expr) : Option Collection :=
+  match_expr e with
+  | Vector.mk t sz xs _ => do return ⟨←CollectionType.mkVec t sz, ←listExprOfArrayExpr xs⟩
+  | Array.mk  t    _    => do return ⟨←CollectionType.mkArray t, ←listExprOfArrayExpr e⟩
+  -- `List.toArray` should not be necessary, as reducible definitions must be reduced first
+  | List.toArray t _    => do
+    dbg_trace s!"`List.toArray` encountered; this is a bug"
+    return ⟨←CollectionType.mkArray t, ←listExprOfArrayExpr e⟩
+  | List.cons t    _  _ => do return ⟨←CollectionType.mkList t, e⟩
+  | List.nil  t         => do return ⟨←CollectionType.mkList t, e⟩
+  | _                   => .none
+  where
+    listExprOfArrayExpr (e : Expr) : Option Expr := do
+      let_expr Array.mk _ l := e | .none
+      .some l
+
+def Collection.cast (coll : Collection) (t : CollectionKind) : Option Collection := do
+  return {coll with type := ←coll.type.cast t}
+
+-- /--
+-- Currently separate from the `vectorElemsOfMk` chain.
+-- -/
+-- def elemsOfColl (e : Expr) : Option (Collection × Array Expr × Expr) :=
+--   match_expr e with
+--   | Vector.mk t sz _ _ => (.Vector t sz, ·) <$> (vectorElemsOfMk e)
+--   | Array.mk t _      => arrayElemsOfExpr' e >>= fun res ↦ .some (.Array t, spoon res)
+--   | _                 => listElemsOfExpr' e >>= fun res ↦ .some (.List, spoon res)
+--   where spoon := fun (arr, t, sz) ↦ (arr, t, toExpr sz)
+
+def Collection.elemsOfExpr (e : Expr) : Option (Array Expr × Collection) :=
+  Collection.elems <$> Collection.ofExpr e
+
+def _root_.Lean.Expr.listLitIsEmpty (e : Expr) : Bool :=
+  match_expr e with
+  | List.cons _ _ _ => false
+  | _ => true
+
+def _root_.Lean.Expr.listLitHead (e : Expr) : Option Expr :=
+  match_expr e with
+  | List.cons _ hd _ => .some hd
+  | _ => .none
+
+def _root_.Lean.Expr.listLitTail (e : Expr) : Option Expr :=
+  match_expr e with
+  | List.cons _ _ tl => .some tl
+  | _ => .none
+
+def explode : MetaM Methods := do
+  return {
+    -- post := explodeVector
+    pre  := dontExplodeVector >> explodeVector
+  }
+
+open Collection in
+/--
+TODO: Probably return the ground size?
+
+Sequenced collection, e.g.:
+- `List.cons a (List.cons b List.nil)` ==> `[a, b]`
+
+Vectors are special, i.e.:
+- `x : Vector τ sz` ==> `[x[0], x[1], ..., x[sz-1]`
+
+We permit any free variable of type vector with size we can reduce to ground nat.
+Unsized collections better enumerate their elements in the first place.
+-/
+def sequenced (e : Expr) : Sym.Simp.SimpM (Option (Array Expr × Collection)) := do
+  match_expr e with
+  | List.cons _ _ _   => return elemsOfExpr e
+  | List.nil  _       => return elemsOfExpr e
+  | Array.mk  _ _     => return elemsOfExpr e
+  | Vector.mk _ _ _ _ => return elemsOfExpr e
+  | _ =>
+    if !e.isFVar then return .none
+    let_expr Vector t sz := ←Sym.inferType e | return .none
+    elemsOfExpr <$> sequenceAsVecExpr e t sz
+
+def _root_.Lean.Expr.foldlM? (e : Expr) : Option (List Expr) :=
+  match_expr e with
+  | Vector.foldlM _ β α _ _ f init xs => .some [α, β, f, init, xs]
+  | Array.foldlM α β _ _ f init xs _ _ => .some [α, β, f, init, xs]
+  | List.foldlM _ _ β α f init xs => .some [α, β, f, init, xs]
+  | _ => .none
+
+def _root_.Lean.Expr.foldlMInfo? (e : Expr) : Option (List Expr) :=
+  match_expr e with
+  | Vector.foldlM m β α _ inst f init xs => .some [m, inst, α, β, f, init, xs]
+  | Array.foldlM α β m inst f init xs _ _ => .some [m, inst, α, β, f, init, xs]
+  | List.foldlM m inst β α f init xs => .some [m, inst, α, β, f, init, xs]
+  | _ => .none
+
+/-
+`a >>= λ a₁ : t₁ ↦ b >>= λ a₂ : t₂ ↦ c >>= λ a₃ : t₃ ↦ a₄ : m t₄` = `(#[(a, t₁), (b, t₂), (c, t₃)], t₄)`
+-/
+partial def _root_.Lean.Expr.sequenceBinds (e : Expr) : Array (Expr × Expr) :=
+  go e #[]
+  where
+    go (e : Expr) (res : Array (Expr × Expr)) :=
+    match_expr e with
+    | Option.bind _ _ a f =>
+      -- The upcoming lambda knows the type of `a`, insert a _dummy_
+      go f (res.push (a, default))
+    | _ =>
+      match e with
+      | .lam _ dom body _ =>
+        let (a, _dummy) := res.back!
+        -- We know the type of `a`, replace the _dummy_
+        go body (res.take (res.size - 1) |>.push (a, dom))
+      | _ =>
+        res.push (e, default)
 
 def mk_append_mk : Simproc := fun e ↦ do
   let_expr HAppend.hAppend _ _ _ _ xs ys := e | return .rfl
 
-  let some (xs, tXs, szXs) := elemsOfColl xs | return .rfl
-  let some (ys, _tYs, szYs) := elemsOfColl ys | return .rfl
-  -- `tXs = _tYs`
-  let result ← Sym.mkListLit tXs (xs.append ys).toList
+  let .some ⟨xsElems, xsC⟩ ← sequenced xs | return .rfl
+  let .some ⟨ysElems, ysC⟩ ← sequenced ys | return .rfl
 
+  let append := xsElems.append ysElems
+
+  -- `xs.type.t = ys.type.t` ∧ `xs.type.k = ys.type.k`
+  let .some appendListColl := Collection.ofExpr (←Sym.mkListLit xsC.type.t append.toList) | unreachable!
   let instAdd := Expr.const ``instAddNat []
-  let inst := mkApp2 (.const ``instHAdd [0]) q(ℕ) instAdd
-
-  let e' ← mkVecLit tXs result (mkApp6 (.const ``HAdd.hAdd [0, 0, 0]) q(ℕ) q(ℕ) q(ℕ) inst szXs szYs)
+  let inst ← shareCommonInc <| mkApp2 (.const ``instHAdd [0]) q(ℕ) instAdd
+  let .some szXs := xsC.type.sz | unreachable!
+  let .some szYs := ysC.type.sz | unreachable!
+  let sz := mkApp6 (.const ``HAdd.hAdd [0, 0, 0]) q(ℕ) q(ℕ) q(ℕ) inst szXs szYs
+  let .some appendVecColl := appendListColl.setSize sz |>.cast xsC.type.k | unreachable!
+  let e' ← appendVecColl.toExpr
 
   trace[Clap.Compile.simp.proc.vector_mk_append_mk]
     m!"\n{e}\n==>\n{e'}"
-  
-  return .step e' (←mkSorry (←mkEq e e') false)
 
-def appendDbg : Sym.Simp.Simproc := fun e ↦ do
-  let_expr HAppend.hAppend _ _ _ _ xs ys := e | return .rfl
-  logInfo m!"DBG:\n{e}"
-  let thm ← mkTheoremFromDecl ``Vector.mk_append_mk
-  match ←thm.pattern.match? e with
-  | .none => logInfo m!"{bombEmoji} Pattern:\n{thm.pattern.pattern}"
-  | .some arr => logInfo m!"{checkEmoji} Matched:\n{arr.args}"
-  logInfo m!"TRY AGAIN: {(← Sym.unfoldReducible e)}"
-  match ←thm.pattern.match? (← Sym.unfoldReducible e) with
-  | .none => logInfo m!"{bombEmoji} Pattern:\n{thm.pattern.pattern}"
-  | .some arr => logInfo m!"{checkEmoji} Matched:\n{arr.args}"
-  return .rfl
+  return .step e' (←mkSorry (←mkEq e e') false)
 
 def append : MetaM Methods :=
   mkPostMethods #[
-    ``Vector.mk_append_mk--, ``List.append_toArray,
-
-    -- ``List.cons_append, ``List.nil_append, ``List.append_nil,
-
-    -- ``Compiler.explodeVectorAppend,
-
-    -- ``appendDbg
+    ``Vector.mk_append_mk
   ]
 
-def explode : MetaM Methods := do
-  return {
-    post := explodeVector
-    pre  := dontExplodeVector
-  }
+/-
+do let x : t₁ ← a1
+   a2
+   let x ← do a3; a4; return 4
+   a3 x
+-/ --> [(a1, t₁), (a2, t₂), (a3, t₃), (a4, t₄), (return 4, ℕ), a3]
+
+partial def _root_.Lean.Expr.sequenceBindsL (e : Expr) : Array (Expr × Expr) :=
+  go #[e] #[]
+where
+  go (todo : Array Expr) (done : Array (Expr × Expr)) : Array (Expr × Expr) :=
+    match todo.back? with
+    | .none => done
+    | .some e =>
+      let todo := todo.pop
+      match e.matchBindsE with
+      | .some (action, func) =>
+        match action.matchBindsE with
+        | .some (b, g) =>
+          go (todo.append #[func, g, b]) done
+        | _ =>
+          go (todo.push func) (done.push (action, default))
+      | _ =>
+        match e with
+        | .lam _ dom body _ =>
+          let done := done.modify done.size.pred fun (a, _) ↦ (a, dom)
+          go (todo.push body) done
+        | _ =>
+          go todo (done.push (e, default))
+
+-- partial def _root_.Lean.Expr.sequenceBindsL (e : Expr) : Array (Expr × Expr) :=
+--   go #[e] #[]
+-- where
+--   go (todo : Array Expr) (done : Array (Expr × Expr)) : Array (Expr × Expr) :=
+--     match todo.back? with
+--     | .none => done
+--     | .some e =>
+--       let todo := todo.pop
+--       match_expr e with
+--       | Option.bind _ _ a f =>
+--         match_expr a with
+--         | Option.bind _ _ b g =>
+--           go (todo.push f |>.push g |>.push b) done
+--         | _ =>
+--           go (todo.push f) (done.push (a, default))
+--       | _ =>
+--         match e with
+--         | .lam _ dom body _ =>
+--           let done := done.modify done.size.pred fun (a, _) ↦ (a, dom)
+--           go (todo.push body) done
+--         | _ =>
+--           go todo (done.push (e, default))
+
+
+-- partial def _root_.Lean.Expr.sequenceBindsL (e : Expr) : Array (Expr × Expr) :=
+--   go e #[]
+--   where
+--     go (e : Expr) (res : Array (Expr × Expr)) :=
+--     match_expr e with
+--     | Option.bind _ _ a f =>
+--       -- TODO: TR the L-traverse
+--       match_expr a with
+--       | Option.bind _ _ b g =>
+--         let res' := go b res
+--         let res'' := go g res'
+--         go f res''
+--       | _ =>
+--         -- The upcoming lambda knows the type of `a`, insert a _dummy_
+--         go f (res.push (a, default))
+--     | _ =>
+--       match e with
+--       | .lam _ dom body _ =>
+--         let (a, _dummy) := res.back!
+--         -- We know the type of `a`, replace the _dummy_
+--         go body (res.pop.push (a, dom))
+--       | _ =>
+--         res.push (e, default)
+
+
+
+-- (bind (bind (b : Option α) (g : α → Option β) : Option β) (f : β → Option γ) : Option γ)
+-- TODO: use `chainActions`
+def bindMyAssoc : Sym.Simp.Simproc := fun e ↦ do
+  let_expr Option.bind β γ a f := e | return .rfl
+  let_expr Option.bind α β b g := a | return .rfl
+  let actions := a.sequenceBinds
+  if actions.isEmpty then throwError m!"empty nested do block"
+  let actions := actions.modify actions.size.pred fun (e, _) ↦ (e, γ)
+  let .lam _ _ body _ := f | throwError m!"expected lambda"
+  let (e', _) ← actions.foldrM (init := (body, γ)) fun (a₁, ta₁) (a₂, ta₂) ↦
+    bindActions a₁ ta₁ a₂ ta₂
+  -- let (e', time) ← timeS (Sym.shareCommon e')
+  -- logInfo m!"sharing took: {time}s"
+  let e ← Sym.shareCommon e'
+  return .step e' (←mkSorry (←mkEq e e') false)
+
+def bindMyAssoc_set : MetaM Methods :=
+  mkPostMethods #[
+    ``bindMyAssoc
+  ]
+
+def monads! : MetaM Sym.Simp.Methods :=
+  mkPreMethods #[
+    ``SymSets.General.monad, ``bindMyAssoc
+  ]
+
+opaque eq0 (n : Nat) : Option Unit
+
+-- circuit (vec : Vector 2 Nat)...
+-- let x : List Nat := f x
+
+/--
+This is for the custom traversal.
+
+TODO(untested, perf, needs restructuring)
+-/
+def foldlM_singlePass : Sym.Simp.Simproc := fun e ↦ do
+  let .some [α, β, f, init, xs] := e.foldlM? | return .rfl
+  /-
+  TODO(perf): With head|tail reasoning, we don't need to traverse the full list literal expr.
+              Using `sequenced` does just that.
+  -/
+  let .some (elems, ⟨⟨_, k, .some sz⟩, listExpr⟩) ← sequenced xs | return .rfl
+  let szSimped := (←Sym.simpWithGround sz).getResultExpr sz
+  match szSimped.nat? with
+  | .none => throwError m!"{sz} does not simplify to ground. Expr:\n{e} (TODO: Maybe this is ok.)"
+  | .some _szSimpedNat => -- TODO(check)
+    let u ← Sym.getLevelInType β
+    let v ← Sym.getLevelInType α
+    let w := u -- `Option : Type u ↦ Type u` preserves the universe
+    match elems with
+    | ⟨[]⟩ =>
+      let e' ← Sym.shareCommonInc <| mkAppN (.const ``Option.some [u]) #[β, init]
+      return .step e' (←mkSorry (←mkEq e e') false) (done := true)
+    | ⟨.cons x _xs⟩ =>
+      -- `f init x`
+      let head ← Sym.shareCommonInc <| mkApp2 f init x
+      -- `_xs` but as list literal
+      let .some xs := listExpr.listLitTail | unreachable!
+      -- TODO(check): I _think_ I got the universes right.
+      -- `List.foldlM f acc xs` where `acc` comes from the enclosing bind
+      let tail ← Sym.shareCommonInc <| mkApp3 (.const ``List.foldlM [u, w, v]) f (.bvar 0) xs
+      -- `bind head tail`
+      let bind ← Sym.shareCommonInc <| mkApp2 (.const ``Option.bind [v, u]) head tail
+      return .step bind (←mkSorry (←mkEq e bind) false)
+
+/--
+`[1, 2, 3, 4].foldlM f b` ==>
+`f b 1 >>= λ next → f next 2 >>= λ next → f next 3 >>= λ next ↦ pure next`
+-/
+def unfold_generic_mk_foldlM : Sym.Simp.Simproc := fun expr ↦ do
+  let .some [inputType, outputType, f, init, collection] := expr.foldlM? | return .rfl
+  let .some (elems, ⟨⟨_, _, .some size⟩, _⟩) ← sequenced collection | return .rfl
+
+  trace[Clap.Compile.dbg]
+    m!"Unfold_generic_mk_foldlM\nelems:{elems}\nsize:{size}"
+
+  let u ← Sym.getLevelInType outputType
+  let v ← Sym.getLevelInType inputType
+
+  let szSimped := (←Sym.simpWithGround size).getResultExpr size
+  match szSimped.nat? with
+  | .none => throwError m!"{size} does not simplify to ground. Expr:\n{expr} (TODO: Maybe this is ok.)"
+  | .some 0 =>
+    -- For an empty collection, return some init
+    let expr' ← Sym.shareCommonInc <| mkAppN (.const ``Option.some [u]) #[outputType, init]
+    trace[Clap.Compile.dbg]
+      m!"Unfold_generic_mk_foldlM 0 branch\nexpr':{expr'}"
+    trace[Clap.Compile.dbg]
+      m!"\n{expr}\n==>\n{expr'}"
+    return .step expr' (←mkSorry (←mkEq expr expr') false)
+  | .some _szSimpedNat => -- TODO(check)
+    -- some next
+    let chain_base ← Sym.shareCommonInc <| mkAppN (.const ``Option.some [u]) #[outputType, .bvar 0]
+
+    -- repeated (f x elem).bind fun x => acc
+
+    let chain := elems.foldr (
+      λ (elem: Expr) (acc: Expr) =>
+        let bind_lhs := mkApp2 f (.bvar 0) elem
+        let bind_rhs := Expr.lam `next outputType acc .default
+        let bind := mkApp4 (.const `Option.bind [v, u]) inputType outputType bind_lhs bind_rhs
+        bind
+    ) chain_base
+
+    let wrapped_chain := Expr.lam `init outputType chain .default
+
+    -- trace[Clap.Compile.dbg]
+    --   m!"Unfold_generic_mk_foldlM init: {init} elems: {elems} wrapped_chain: {wrapped_chain}"
+
+    let reduced_chain := wrapped_chain.beta #[init]
+
+    -- trace[Clap.Compile.dbg]
+    --   m!"Unfold_generic_mk_foldlM reduced_chain: {reduced_chain}"
+
+    let expr' ← Sym.shareCommonInc <| reduced_chain
+
+
+    trace[Clap.Compile.dbg]
+      m!"\n{expr}\n==>\n{expr'}"
+
+    return .step expr' (←mkSorry (←mkEq expr expr') false)
+
+/--
+  `#v[a₁, a₂, ...].foldlM (init := x) f`
+  `f a₁ x >>= fun rest ↦ [a₂, ...].foldlM (init := rest) f`
+-/
+def foldlM_stagger : Sym.Simp.Simproc := fun e ↦ do
+  let .some [m, inst, α, β, f, init, collection] := e.foldlMInfo? | return .rfl
+  -- TODO(perf): `coll` not necessary in full
+  let .some ⟨_, listExpr⟩ := Collection.ofExpr collection | return .rfl
+  -- let us@([u, v, w]) := e.getAppFn.constLevels! | unreachable!
+  let u₁ ← Sym.getLevelInType β
+  let u₂ := u₁
+  let u₃ ← Sym.getLevelInType α
+  let listFold ← Sym.shareCommonInc <|
+    mkApp7
+      (.const ``List.foldlM [u₁, u₂, u₃])
+      m inst 
+      β α f init listExpr
+  match_expr listExpr with
+  | List.cons _ hd tl =>
+    -- let theorems : Theorems := ({} : Theorems).insert (←mkTheoremFromDecl ``List.foldlM_cons)
+    -- let e' ← theorems.rewrite dischargeNone listFold
+    -- let e' := e'.getResultExpr e
+    let head ← Sym.shareCommonInc <| f.beta #[init, hd]
+    let tail ← Sym.shareCommonInc <| mkApp7 (.const ``List.foldlM [u₁, u₂, u₃])
+                                            m inst
+                                            β α f (.bvar 0) tl
+    let lambda ← Sym.shareCommonInc <| .lam `next β tail .default
+    -- TODO(perf): Hand-write the types I guess vOv.
+    let tailτ ← Sym.inferType tail
+    let tailτu ← Sym.getLevelInType tailτ
+    let e' ← Sym.shareCommonInc <| mkApp4 (.const ``Option.bind [u₁, tailτu]) β tailτ head lambda
+    trace[Clap.Compile.simp.proc.vector_foldlM_stagger]
+      m!"\n{e}\n==>\n{e'}"
+    let e' ← Sym.shareCommonInc <| Simp.wrapped (←Sym.inferType e') e'
+    return .step e' (←mkSorry (←mkEq e e') false) (done := true)
+  | _ =>
+    let e' := mkApp2 (.const ``Option.some [u₁]) β init
+    trace[Clap.Compile.simp.proc.vector_foldlM_stagger]
+      m!"\n{e}\n==>\n{e'}"
+    return .step e' (←mkSorry (←mkEq e e') false) (done := true)
 
 def foldlM : MetaM Methods :=
-  mkPostMethods #[
+  mkPreMethods #[
     ``Vector.foldlM_mk, ``List.foldlM_toArray,
 
     ``List.foldlM_cons, ``List.foldlM_nil
   ]
 
-def getElemDbg : Sym.Simp.Simproc := fun e ↦ do
-  logInfo m!"getElemDbg: {e}"
-  let_expr GetElem.getElem _ _ _ _ _ coll i h := e | return .rfl
-  logInfo m!"coll: {coll}\ni: {i}"
-  let_expr Vector.mk _ _ arr h := coll |
-    logInfo m!"Rejected: {coll}"
-    logInfo m!"App of: {coll.getAppFnArgs}"
-    return .rfl
-  logInfo m!"arr: {arr}"
-  logInfo m!"This is getElem on Vector.mk:\n({coll})[{i}]"
-  logInfo m!"e:\n{e}"
-  
-  let thm ← mkTheoremFromDecl ``Vector.getElem_mk
-  logInfo m!"thm pattern: {thm.pattern.pattern}"
+-- def foldlM_mk_post : MetaM Methods :=
+--   mkPostMethods #[
+--     ``foldlM_mk
+--   ]
 
-  match ← thm.pattern.match? e with
-  | .none => logInfo m!"NO MATCH:\n{e}\n=?=\n{thm.pattern.pattern}"
-  | .some e' => logInfo m!"YOU TRIGGERED SON! OK!: {e'.args}"
+def foldlM_singlePass_s : MetaM Methods :=
+  mkPreMethods #[
+    ``foldlM_singlePass
+  ]
 
-  return .rfl
+def foldlM_post : MetaM Methods :=
+  mkPostMethods #[
+    ``Vector.foldlM_mk, ``List.foldlM_toArray,
 
--- private def getElem_t : Simproc := fun e ↦ do
---   let_expr GetElem.getElem collT _ _ _ _ coll i h := e | return .rfl
---   let_expr Vector _ sz := collT | return .rfl
---   let simpedSz := (←Sym.simp sz (←General.ground)).getResultExpr sz
---   match simpedSz.nat? with
---   | .none => return .rfl
---   | .some simpedSzN =>
---     return .rfl
---     -- if simpedSz == sz then return .rfl -- TODO: `isSameExpr`?
---     -- let coll ← cowboyCast coll simpedSzN
---     -- let e' := ←mkAppM ``GetElem.getElem #[coll, i]
---     -- logInfo m!"e': {e'}"
---     -- -- This plays loose, let's pretend this is ok for now.
---     -- return .step e' (←mkSorry (←mkEq e e') false)
---     -- logInfo m!"szVec: {(←Sym.simp sz (←General.ground)).getResultExpr sz}"
---     -- logInfo m!"szVecSimped: {sz}"
---     -- let_expr Vector.mk _ sz arr _ := coll | return .rfl
-
---     -- logInfo m!"sz: {sz}"
---     -- logInfo m!"simped sz: {(←Sym.simp sz).getResultExpr sz}"
---     -- return .rfl
-
--- /--
--- `Vector.getElem_mk` up to reducible.
--- Trying to be as explicit as possible for `Sym`.
--- -/
--- private def getElem_mk : Simproc := fun e ↦ do
---   let_expr GetElem.getElem collT _ _ _ _ coll i h := e | return .rfl
---   let_expr Vector _ _getElemSz := collT | return .rfl
---   let_expr Vector.mk _ _mkSz arr _ := coll | return .rfl
---   -- Note we are not looking at `_getElemSz` and `_mkSz`.
---   logInfo m!"WAT {h}"
---   let szProof ← mkLt i (←mkAppM ``Array.size #[arr])
---   let e' ← mkAppM ``GetElem.getElem #[arr, i, ←mkSorry szProof false]
---   trace[Clap.Compile.simp.proc.getElem_mk] m!"{e}\n==>\n{e'}"
---   return .step e' (←mkSorry (←mkEq e e') false)
---   -- let getElemSz := (←Sym.simp getElemSz (←General.ground)).getResultExpr getElemSz
---   -- let mkSz := (←Sym.simp mkSz (←General.ground)).getResultExpr mkSz
---   -- unless isSameExpr getElemSz mkSz do return .rfl
---   -- trace[Clap.Compile.simp.proc.getElem_mk] m!""
-  -- _
-
--- #check Vector.getElem_mk
--- def getElem_mk : Sym.Simp.Simproc := fun e ↦ do
---   let_expr GetElem.getElem collT _ _ _ _ coll _ _ := e | return .rfl
---   let_expr Vector.mk _ sz arr _ := coll | return .rfl
---   let_expr Vector _ getElemSz := collT | return .rfl
---   logWarning m!"Doing.\nGetElem={getElemSz}\nVec.mk={sz}"
---   if isSameExpr getElemSz sz then -- `1 + 1 ≠ 2`
---     let thm ← mkTheoremFromDecl ``Vector.getElem_mk -- TODO: Don't do this lazily here.
---     let e' ← thm.rewrite e
---     trace[Clap.Compile.simp.proc.vector_getElem_mk]
---       m!"\n{e}\n==>\n{e'.getResultExpr e}"
---     return e'
---   let simpedSz := (←Sym.simp sz (←General.ground)).getResultExpr sz
---   match simpedSz.nat? with
---   | .none =>
---     throwError m!"{simpedSz} is not ground.\nMaybe this is ok."
---     return .rfl
---   | .some simpedSzN =>
---     logInfo m!"sz:{sz}\nsimpedSz: {(←Sym.simp sz (←General.ground)).getResultExpr sz}"
---     let e' ← inferVectorProof (←mkAppM ``GetElem.getElem #[arr, mkNatLit simpedSzN]) -- GetElem (Array Nat)
---     let e' ← Compiler.Simp.reducedAndSharedInc e'
---     trace[Clap.Compile.simp.proc.vector_getElem_mk]
---       m!"\n{e}\n==>\n{e'}\nCheating.\nIn {collT} we pretend that {getElemSz} = {simpedSzN}."
---     return .step e' (←mkSorry (←mkEq e e') false)
--- -- Vector.append : Vec m ++ Vec n ==> Vec (m + n) ==> Vec k where k = n + n
--- -- do let x := (vec ++ vec)[1] -- (vec ++ vec : Vector (m + n)) -- GetElem (Vector (3 + 3)) 
--- #check Vector.append
--- #check GetElem.getElem (coll := Vector ℕ 4) (Vector.mk (n := 2 + 2) #[1, 2, 3, 4] rfl) 0 (by decide)
+    ``List.foldlM_cons, ``List.foldlM_nil
+  ]
 
 def getElem_mk : Sym.Simp.Simproc := fun e => do
   -- In vector, we can optimise by not enumerating all elements first,
@@ -468,12 +939,17 @@ def getElem_mk : Sym.Simp.Simproc := fun e => do
 
   -- Instead, we can simply traverse the first `i` conses, as we have the length apriori for the proof.
   -- Or some such.
-  let_expr GetElem.getElem _ _ _ _ _ vec n _ := e | return .rfl
-  let some (elems, _, sz) := elemsOfColl vec | return .rfl
-  -- let some (elems, _, sz) := vectorElemsOfMk vec | return .rfl
-  let some i := Sym.getNatValue? n | return .rfl
-  trace[Clap.Compile.simp.proc.vector_getElem_mk]
-    m!"Info:\nVector size: {sz}\nElems size: {elems.size}"
+  let_expr GetElem.getElem _ _ _ _ _ vec n _ := e |
+    -- trace[Clap.Compile.simp.proc.vector_getElem_mk]
+    --   m!"rejected: {e}"
+    return .rfl
+  let .some (elems, t) := Collection.elemsOfExpr vec |
+    -- trace[Clap.Compile.simp.proc.vector_getElem_mk]
+    --   m!"rejected: {e}"
+    return .rfl
+  let .some sz := t.type.sz | unreachable!
+  let n := (←Sym.simpWithGround n).getResultExpr n
+  let .some i := Sym.getNatValue? n | return .rfl
   if h : i < elems.size
   then
     let e' := elems[i]
@@ -497,48 +973,34 @@ def getElem : MetaM Methods :=
 
 def getElem_old : MetaM Methods :=
   mkPostMethods #[
-    -- ``getElem_t,
     ``Vector.getElem_mk, ``List.getElem_toArray,
 
     ``List.getElem_cons_zero, ``List.getElem_cons_succ,
-
-    -- ``getElemDbg
   ]
-
-def mapDbg : Sym.Simp.Simproc := fun e ↦ do
-  let_expr Array.map _ _ _ _ := e | return .rfl
-  logInfo m!"Is Array.map:\n{e}"
-  let thm ← mkTheoremFromDecl ``List.map_toArray
-  match ←thm.pattern.match? e with
-  | .none => logInfo m!"{bombEmoji} Pattern:\n{thm.pattern.pattern}"
-  | .some e => logInfo m!"{checkEmoji} Pattern:\n{e.args}"
-  match ←thm.pattern.match? (←Compiler.Simp.preprocessExpr e) with
-  | .none => logInfo m!"{bombEmoji} Pattern:\n{thm.pattern.pattern}"
-  | .some e => logInfo m!"{checkEmoji} Pattern:\n{e.args}"
-  return .rfl
 
 def map : MetaM Methods :=
   mkPostMethods #[
     ``Vector.map_mk, ``List.map_toArray,
-    
-    ``List.map_cons, ``List.map_nil,
 
-    -- ``Compiler.explodeVectorMap
+    ``List.map_cons, ``List.map_nil,
   ] ∪ mapOptim
   where
     mapOptim : MetaM Methods := mkPreMethods #[``List.map_id]
 
 def mapIdx_mk : Sym.Simp.Simproc := fun e => do
   let_expr Vector.mapIdx _ β sz f xs := e | return .rfl
-  let some (xs, _) := vectorElemsOfMk xs | return .rfl
+  let some (xs, _) := vectorElemsOfMk xs |
+    trace[Clap.Compile.simp.proc.vector_mapIdx_mk]
+      m!"rejected:\n{e}"
+    return .rfl
 
   let result ← Sym.mkListLit β (xs.mapIdx (f.beta #[mkNatLit ·, ·])).toList
   let e' ← mkVecLit β result sz
 
   trace[Clap.Compile.simp.proc.vector_mapIdx_mk]
     m!"\n{e}\n==>\n{e'}"
-  
-  return .step e' (←mkSorry (←mkEq e e') false) 
+
+  return .step e' (←mkSorry (←mkEq e e') false)
 
 def mapIdx : MetaM Methods :=
   mkPostMethods #[
@@ -550,6 +1012,24 @@ def listOfArray (e : Expr) : Option Expr :=
   then .none
   else .some e.getAppArgs[1]!
 
+def _root_.Lean.Expr.mapM? (e : Expr) : Option (List Expr) :=
+  match_expr e with
+  | Vector.mapM _ α β _ _ f xs => .some [f, α, β, xs]
+  | Array.mapM α β _ _ f xs    => .some [f, α, β, xs]
+  | List.mapM _ _ α β f xs     => .some [f, α, β, xs]
+  | _                          => .none
+
+/--
+TODO: No `MetaM` or better, how do I grab the universe of `α`?
+      Of course we can just return `m n` from this, infer the `Sort` of `α` in the caller
+      and reconstruct the `Vector` typpe this way, but it would make the interface of this dreary.
+-/
+def _root_.Lean.Expr.append? (e : Expr) : Option (List Expr) :=
+  match_expr e with
+  | HAppend.hAppend α β γ _ xs ys => .some [α, β, γ, xs, ys]
+  | _root_.Vector.append _ _ _ _ _ => panic! "Vector.append not implemented yet."
+  | _ => .none
+
 open Compiler.Simp in
 /--
 Single step transformation. TODO: Does not play particularly nice with our top-level driver.
@@ -557,11 +1037,8 @@ Single step transformation. TODO: Does not play particularly nice with our top-l
 `f x₀ >>= fun row₀ ↦ f x₁ >>= fun row₁ ↦ ... fun rowₘ ↦ .some #v[row₀, row₁, ..., rowₘ]`
 -/
 def _root_.Vector.mapM_mk : Sym.Simp.Simproc := fun e ↦ do
-  let time ← IO.monoMsNow
-  let_expr _root_.Vector.mapM _ α β sz _ f vec := e | return .rfl
-  -- Ultimately, only `Vector.mk` is permitted. Free variables are transformed first.
-  let vec ← if vec.isFVar then sequenceAsVecExpr vec α sz else pure vec
-  if !vec.isAppOf ``Vector.mk then return .rfl
+  let .some [f, _, β, xs] := e.mapM? | return .rfl
+  let .some (elems, ⟨⟨_, k, .some sz⟩, _⟩) ← sequenced xs | return .rfl
   let szSimped := (←Sym.simpWithGround sz).getResultExpr sz
   if !isSameExpr sz szSimped then
     trace[Clap.Compile.simp.proc.vector_mapM_mk]
@@ -570,25 +1047,28 @@ def _root_.Vector.mapM_mk : Sym.Simp.Simproc := fun e ↦ do
   | .none => throwError m!"{sz} does not simplify to ground. Expr:\n{e} (TODO: Maybe this is ok.)"
   | .some szSimpedNat =>
     let transformedList ← Sym.mkListLit β <| (List.range szSimpedNat).reverse.map .bvar
-    let transformedVector ← mkVecLit β transformedList szSimped
-    let transformedVectorT ← Sym.inferType transformedVector
-    let v ← Sym.getLevelInType transformedVectorT
-    let transformedVector? :=
-      mkAppN (.const ``Option.some [v]) #[←Sym.inferType transformedVector, transformedVector]
-    let transformedVector? ← Sym.shareCommonInc transformedVector?
-    let .some (elems, _) := vectorElemsOfMk vec | unreachable!
+    let .some transformedColl :=
+      Collection.ofExpr transformedList <&>
+      Collection.setSize (sz := szSimped) >>=
+      Collection.cast (t := k) | unreachable!
+    let transformedColl ← transformedColl.toExpr
+    let transformedCollT ← Sym.inferType transformedColl
+    let v ← Sym.getLevelInType transformedCollT
+    let transformedColl? :=
+      mkAppN (.const ``Option.some [v]) #[transformedCollT, transformedColl]
+    let transformedColl? ← Sym.shareCommonInc transformedColl?
     let u ← Sym.getLevelInType β
     /-
     Start with `.some #[.bvar sz.pred, .bvar sz.pred.pred, ..., .bvar 0]`
     Prefix a single lambda in each iteration.
     -/
-    let e' ← (List.range szSimpedNat).foldrM (init := transformedVector?) fun i e ↦ do
+    let e' ← (List.range szSimpedNat).foldrM (init := transformedColl?) fun i e ↦ do
       let elem := elems[i]!
       liftM ∘ Sym.shareCommonInc <|
         mkAppN                                         -- `f vec[i] >>= fun row_{i} ↦ e`
           (.const ``Option.bind [u, v])
           #[
-            β, transformedVectorT,                     -- implicits
+            β, transformedCollT,                       -- implicits
             ←Sym.shareCommonInc (f.beta #[elem]),      -- `f vec[i]`
             .lam (binderInfo := .default)
                  (binderName := .mkSimple s!"row_{i}")
@@ -596,11 +1076,336 @@ def _root_.Vector.mapM_mk : Sym.Simp.Simproc := fun e ↦ do
                  (body       := e)                     -- `fun row_{i} ↦ e`
           ]
       -- Careful, `e` contains loose bvars until the very last iteration.
-    trace[Clap.Compile.simp.proc.vector_mapM_mk_cons]
+    trace[Clap.Compile.simp.proc.vector_mapM_mk]
       m!"\n{e}\n==>\n{e'}"
     let proof ← mkSorry (←mkEq e e') false
-    Dbg.timeSince time "Vector.mapM_mk_cons took"
+    -- Dbg.timeSince time "mapM_mk_cons took:"
     return .step e' proof
+
+open Compiler.Simp in
+/--
+Single step transformation. TODO: Does not play particularly nice with our top-level driver.
+`Vector.mapM f #v[x₀, x₁, ..., xₘ]` ==>
+`f x₀ >>= fun row₀ ↦ f x₁ >>= fun row₁ ↦ ... fun rowₘ ↦ .some #v[row₀, row₁, ..., rowₘ]`
+-/
+def _root_.Vector.mapM_mk_seq : Sym.Simp.Simproc := fun e ↦ do
+  let .some [f, _, β, xs] := e.mapM? | return .rfl
+  let .some (elems, ⟨⟨_, k, .some sz⟩, _⟩) ← sequenced xs | return .rfl
+  let szSimped := (←Sym.simpWithGround sz).getResultExpr sz
+  if !isSameExpr sz szSimped then
+    trace[Clap.Compile.simp.proc.vector_mapM_mk]
+      m!"Info: Processing `Vector _ ({sz})` of ground length {szSimped}. Request:\n{e}"
+  match szSimped.nat? with
+  | .none => throwError m!"{sz} does not simplify to ground. Expr:\n{e} (TODO: Maybe this is ok.)"
+  | .some szSimpedNat =>
+    let transformedList ← Sym.mkListLit β <| (List.range szSimpedNat).reverse.map .bvar
+    let .some transformedColl :=
+      Collection.ofExpr transformedList <&>
+      Collection.setSize (sz := szSimped) >>=
+      Collection.cast (t := k) | unreachable!
+    let transformedColl ← transformedColl.toExpr
+    let transformedCollT ← Sym.inferType transformedColl
+    let v ← Sym.getLevelInType transformedCollT
+    let transformedColl? :=
+      mkAppN (.const ``Option.some [v]) #[transformedCollT, transformedColl]
+    let transformedColl? ← Sym.shareCommonInc transformedColl?
+    let u ← Sym.getLevelInType β
+    /-
+    Start with `.some #[.bvar sz.pred, .bvar sz.pred.pred, ..., .bvar 0]`
+    Prefix a single lambda in each iteration.
+    -/
+    let e' ← (List.range szSimpedNat).foldrM (init := transformedColl?) fun i e ↦ do
+      let elem := elems[i]!
+      liftM ∘ Sym.shareCommonInc <|
+        mkAppN                                         -- `f vec[i] >>= fun row_{i} ↦ e`
+          (.const ``Option.bind [u, v])
+          #[
+            β, transformedCollT,                       -- implicits
+            ←Sym.shareCommonInc (f.beta #[elem]),      -- `f vec[i]`
+            .lam (binderInfo := .default)
+                 (binderName := .mkSimple s!"row_{i}")
+                 (binderType := β)
+                 (body       := e)                     -- `fun row_{i} ↦ e`
+          ]
+      -- Careful, `e` contains loose bvars until the very last iteration.
+    trace[Clap.Compile.simp.proc.vector_mapM_mk]
+      m!"\n{e}\n==>\n{e'}"
+    let proof ← mkSorry (←mkEq e e') false
+    -- Dbg.timeSince time "mapM_mk_cons took:"
+    trace[Clap.Compile.simp.proc.vector_mapM_mk]
+      m!"SEQ: {e'.sequenceBindsL}"
+    return .step e' proof
+
+def reportMaxShared (e : Expr) (descr : String := "") : Sym.Simp.SimpM Unit := do
+  try
+    e.checkMaxShared
+    logInfo m!"Is max shared.\n{descr}"
+  catch _ =>
+    logInfo m!"Not max shared.\n{descr}"
+
+/--
+Currently for vectors only.
+
+`Vector.mapM f #v[x, ..v] = do`
+  `let __do_lift ← f x`
+  `let __do_lift_1 ← Vector.mapM f v`
+  `pure (#v[__do_lift] ++ __do_lift_1)`
+-/
+def _root_.Vector.mapM_mk_single : Sym.Simp.Simproc := fun e ↦ do
+  let_expr _root_.Vector.mapM m α β n mInst f vec := e | return .rfl
+  let_expr _root_.Vector.mk _ sz arr _ := vec | return .rfl
+  recordRuleDbg "mapM_mk_single"
+  -- reportMaxShared e (descr := "BEGIN[mapM_mk_single]")
+  let l ← arr.getAppArgs[1]?.getDM (unreachable!)
+  let u ← Sym.getLevelInType β
+  let_expr List.cons t hd tl := l |
+    -- `#v[].mapM f ==> pure #v[]`
+    -- TODO: Check universe
+    let e' := mkApp2
+                (.const ``Option.some [u])
+                (mkApp2 (.const ``Vector [u]) β q(0))
+                (←mkVecLit β (←Sym.mkListLit β []) q(0))
+    trace[Clap.Compile.simp.proc.mapM_mk_single]
+      m!"\n{e}\n==>\n{e'}"
+    return .step e' (←mkSorry (←mkEq e e') false)
+  let sz' ← Sym.simpWithGround sz
+  match (sz'.getResultExpr sz).nat? with
+  | .none => throwError m!"{sz} does not simplify to ground. Expr:\n{e}"
+  | .some szN =>
+    /-
+    No universe bump along the way
+    `Vector.{u} {α : Type u}... : Vector.{u}`
+    -/
+    let v := u
+    let w := u
+
+    let hdSz := mkNatLit 1
+    let tlSz := mkNatLit szN.pred
+
+    -- `#v[__do_lift] ++ __do_lift_1`
+    /-
+      TODO(perf): Use the instance-less one for every typeclass'd operation.
+    -/
+    let append :=
+      mkAppN
+        (.const ``HAppend.hAppend [u, v, w]) #[
+          (mkApp2 (.const ``Vector [u]) β hdSz),
+          (mkApp2 (.const ``Vector [u]) β tlSz),
+          (mkApp2 (.const ``Vector [u]) β (toExpr szN)),
+          (mkApp3 (.const ``Vector.instHAppendHAddNat [u]) β hdSz tlSz),
+          ←mkVecLit β (←Sym.mkListLit β [.bvar 1]) hdSz,
+          .bvar 0
+        ]
+
+    -- let append := mkApp5 (.const ``_root_.Vector.append [u])
+    --                 β hdSz tlSz (←mkVecLit β (←Sym.mkListLit β [.bvar 1]) hdSz) (.bvar 0)
+
+    let tlVec ← mkVecLit α tl tlSz
+
+    -- TODO: Check universes. `Vector` construction should preserve `u`.
+    let v := u
+    let w ← Sym.getLevelInType α
+    let mapM := mkApp7 (.const ``Vector.mapM [u, v, w]) m α β tlSz mInst f tlVec
+    -- TODO(perf): Hand write the type if helps, least of my problems
+    let mapMT ← Sym.inferType mapM
+    let_expr Option mapMT := mapMT | throwError m!"expected Option monad"
+    let appendT ← Sym.inferType append
+    let v ← Sym.getLevelInType mapMT
+
+    let someAppend := mkApp2 (.const ``Option.some [u]) appendT append
+    -- `Vector.mapM f tl >>= fun __do_lift_1 ↦ pure (#v[__do_lift] ++ __do_lift_1)`
+    let innerBind :=
+      mkApp4
+        (.const ``Option.bind [u, v]) mapMT appendT mapM
+        (.lam `_snd mapMT someAppend .default)
+    /-
+    TODO: Check the second universe, it's what `append : Vector.{u} (#[#1] ++ #0)` lives in, I think.
+          Hence `u`. Or so I think.
+    -/
+    /-
+      `let __do_lift ← f x >>= inner`
+    -/
+    let bind :=
+      mkApp4
+        (.const ``Option.bind [u, u])
+        β
+        appendT
+        (←Sym.shareCommonInc (f.beta #[hd])) -- TODO(?): `Expr.app f hdVec` without reducing here?
+        (.lam `fst t innerBind .default )
+    let e' ← Sym.shareCommonInc bind
+    -- let (e', time) ← timeS (Sym.shareCommonInc bind)
+
+    -- logInfo m!"END[mapM_mk_single] Sym.shareCommonInc took {time}s"
+
+    -- reportMaxShared e' (descr := "END[mapM_mk_single]")
+    trace[Clap.Compile.simp.proc.mapM_mk_single]
+      m!"\n{e}\n==>\n{e'}"
+
+    return .step e' (←mkSorry (←mkEq e e') false)
+
+/--
+Currently for vectors only.
+
+`Vector.mapM f #v[x, ..v] = do`
+  `let __do_lift ← f x`
+  `let __do_lift_1 ← Vector.mapM f v`
+  `pure (#v[__do_lift] ++ __do_lift_1)`
+-/
+def _root_.Vector.mapM_mk_single_singlePass : Sym.Simp.Simproc := fun e ↦ do
+  let_expr _root_.Vector.mapM m α β n mInst f vec := e | return .rfl
+  let_expr _root_.Vector.mk _ sz arr _ := vec | return .rfl
+
+  let l ← arr.getAppArgs[1]?.getDM (unreachable!)
+  let u ← Sym.getLevelInType β
+  let_expr List.cons t hd tl := l |
+    -- `#v[].mapM f ==> pure #v[]`
+    let e' := mkApp2 (.const ``Option.some [u]) β (←mkVecLit β (←Sym.mkListLit β []) q(0))
+    trace[Clap.Compile.simp.proc.mapM_mk_single]
+      m!"\n{e}\n==>\n{e'}"
+    return .step e' (←mkSorry (←mkEq e e') false) (done := true)
+  let sz' ← Sym.simpWithGround sz
+  match (sz'.getResultExpr sz).nat? with
+  | .none => throwError m!"{sz} does not simplify to ground. Expr:\n{e}"
+  | .some szN =>
+    /-
+    No universe bump along the way
+    `Vector.{u} {α : Type u}... : Vector.{u}`
+    -/
+    let v := u
+    let w := u
+
+    let hdSz := mkNatLit 1
+    let tlSz := mkNatLit szN.pred
+
+    -- `#v[__do_lift] ++ __do_lift_1`
+    /-
+      TODO(perf): Use the instance-less one for every typeclass'd operation.
+    -/
+    let append :=
+      mkAppN
+        (.const ``HAppend.hAppend [u, v, w]) #[
+          (mkApp2 (.const ``Vector [u]) β hdSz),
+          (mkApp2 (.const ``Vector [u]) β tlSz),
+          (mkApp2 (.const ``Vector [u]) β (toExpr szN)),
+          (mkApp3 (.const ``Vector.instHAppendHAddNat [u]) β hdSz tlSz),
+          ←mkVecLit β (←Sym.mkListLit β [.bvar 1]) hdSz,
+          .bvar 0
+        ]
+
+    let tlVec ← mkVecLit α tl tlSz
+
+    -- TODO: Check universes. `Vector` construction should preserve `u`.
+    let v := u
+    let w ← Sym.getLevelInType α
+    let mapM := mkApp7 (.const ``Vector.mapM [u, v, w]) m α β tlSz mInst f tlVec
+    -- TODO(perf): Hand write the type if helps, least of my problems
+    let mapMT ← Sym.inferType mapM
+    let appendT ← Sym.inferType append
+    let v ← Sym.getLevelInType mapMT
+
+    let someAppend := mkApp2 (.const ``Option.some [u]) appendT append
+
+    -- `Vector.mapM f tl >>= fun __do_lift_1 ↦ pure (#v[__do_lift] ++ __do_lift_1)`
+    let innerBind :=
+      mkApp4
+        (.const ``Option.bind [u, v]) mapMT appendT mapM
+        (.lam `_snd mapMT someAppend .default)
+
+    /-
+    TODO: Check the second universe, it's what `append : Vector.{u} (#[#1] ++ #0)` lives in, I think.
+          Hence `u`. Or so I think.
+    -/
+    /-
+      `let __do_lift ← f x >>= inner`
+    -/
+    let bind :=
+      mkApp4
+        (.const ``Option.bind [u, u])
+        β
+        appendT
+        (←Sym.shareCommonInc (f.beta #[hd])) -- TODO(?): `Expr.app f hdVec` without reducing here?
+        (.lam `fst t innerBind .default )
+
+    -- See the docs of `singlePass`
+    let e' ← Sym.shareCommonInc (singlePass appendT bind)
+
+    trace[Clap.Compile.simp.proc.mapM_mk_single]
+      m!"\n{e}\n==>\n{e'}"
+
+    return .step e' (←mkSorry (←mkEq e e') false) (done := true)
+
+def mapM_singlePass : MetaM Methods :=
+  mkPostMethods #[
+    ``Vector.mapM_mk_single_singlePass
+  ]
+
+def mapM_singlePass_pre : MetaM Methods :=
+  mkPreMethods #[
+    ``Vector.mapM_mk_single_singlePass
+  ]
+
+  -- -- logInfo m!"Nodes: {←e.numObjs}"
+  -- -- let α ← IO.monoMsNow
+  -- let_expr _root_.Vector.mapM _ _ _ _ _ f vec := e | return .rfl
+  -- let_expr _root_.Vector.mk _ sz arr _ := vec | return .rfl
+  -- logInfo m!"e: {e}"
+  -- unless arr.isAppOf ``List.toArray || arr.isAppOf ``Array.mk do return .rfl
+  -- let l ← arr.getAppArgs[1]?.getDM (unreachable!)
+  -- let_expr List.cons t hd tl := l | return .rfl
+  -- let sz' ← Sym.simp sz
+  -- match (sz'.getResultExpr sz).nat? with
+  -- | .none => throwError m!"{sz} does not simplify to ground. Expr:\n{e}"
+  -- | .some szN =>
+  --   if szN == 0 then return .rfl
+  --   let hdVec ← mkVecLit t (←Sym.mkListLit t [hd]) (mkNatLit 1)
+  --   let tl ← mkVecLit t tl (toExpr (szN - 1))
+  --   let appendHdTl ← if szN == 1 then pure hdVec else mkAppM ``HAppend.hAppend #[hdVec, tl]
+  --   let_expr Vector _ szAppendHdTl := ←Sym.inferType appendHdTl | unreachable!
+  --   let szAppendHdTlQ : Q(ℕ) := szAppendHdTl
+  --   let szDesired : Q(ℕ) := toExpr szN
+  --   let proof ← mkSorry q($szAppendHdTlQ = $szDesired) false
+  --   -- logInfo m!"will try to cowboy cast: {appendHdTl}"
+  --   -- let thatGuy ← cowboyCast appendHdTl szN
+  --   let thatGuy := appendHdTl
+  --   let thisGuy := appendHdTl
+  --   let thisGuy := thatGuy
+  --   let mapM ← mkAppM ``_root_.Vector.mapM #[f, thisGuy]
+  --   let theMiddleBit ←
+  --     if szN == 1
+  --     then mkVecLit t (←Sym.mkListLit t [.bvar 1]) (mkNatLit 1)
+  --     else pure <| mkAppN
+  --           (.const ``HAppend.hAppend [
+  --             ←getDecLevel (←Sym.inferType hdVec),
+  --             ←getDecLevel (←Sym.inferType tl),
+  --             ←getDecLevel (←Sym.inferType thisGuy)
+  --           ]) #[
+  --             ←Sym.inferType hdVec,
+  --             ←Sym.inferType tl,
+  --             ←Sym.inferType thisGuy,
+  --             -- ←Sym.inferType appendHdTl,
+  --             ←Sym.synthInstance (←mkAppM ``HAppend #[←Sym.inferType hdVec,←Sym.inferType tl,←Sym.inferType thisGuy,]),
+  --             ←mkVecLit t (←Sym.mkListLit t [.bvar 1]) (mkNatLit 1),
+  --             .bvar 0
+  --           ]
+  --   logInfo m!"theMiddleBit: {theMiddleBit}"
+  --   let consMapM ←
+  --     mkAppM ``Option.bind #[
+  --       f.beta #[hd],
+  --       -- Expr.app f hdVec,
+  --       .lam `fst t
+  --         (←mkAppM ``Option.bind #[
+  --                    ←mkAppM ``Vector.mapM #[f, tl],
+  --                    .lam `snd (←Sym.inferType tl)
+  --                      (←mkAppM ``Option.some #[theMiddleBit])
+  --                      .default
+  --         ])
+  --         .default
+  --     ]
+  --   logInfo m!"consMapM: {consMapM}"
+  --   let e' ← Sym.shareCommonInc consMapM
+  --   trace[Clap.Compile.simp.proc.vector_mapM_mk]
+  --     m!"\n{e}\n==>\n{e'}"
+  --   return .step consMapM (←mkSorry (←mkEq e mapM) false)
 
 /--
 `Vector.mapM_mk_singleton_append` is a part of `Vector.mapM_mk_append` to ensure that
@@ -613,6 +1418,18 @@ def mapM : MetaM Methods :=
     -- ``Compiler.explodeVectorMapM
   ]
 
+def mapM_seq : MetaM Methods :=
+  mkPostMethods #[
+    ``Vector.mapM_mk_seq
+  ]
+
+def mapM_alt : MetaM Methods :=
+  mkPostMethods #[
+    ``Vector.mapM_mk_single
+    -- ``Compiler.explodeVectorMapM
+  ]
+
+#check List.map_cons
 -- def mapM_test : MetaM Methods :=
 --   mkPostMethods #[
 --     ``Vector.mapM_mk_cons, ``Compiler.explodeVectorMapM
@@ -641,14 +1458,14 @@ def mk_zipWith_mk : Sym.Simp.Simproc := fun e => do
 
   trace[Clap.Compile.simp.proc.vector_mk_zipWith_mk]
     m!"\n{e}\n==>\n{e'}"
-  
-  return .step e' (←mkSorry (←mkEq e e') false) 
+
+  return .step e' (←mkSorry (←mkEq e e') false)
 
 def zipWith : MetaM Methods :=
   mkPostMethods #[
     ``Vector.mk_zipWith_mk,
     -- ``List.zipWith_toArray,
-    
+
     -- ``List.zipWith_cons_cons, ``List.zipWith_nil_left, ``List.zipWith_nil_right,
 
     -- ``Compiler.explodeVectorZipWith
@@ -672,10 +1489,19 @@ def drop : MetaM Methods :=
     -- ``Compiler.explodeVectorDrop
   ]
 
+def _root_.List.replicate_toArray {α : Type} {n} {v} := (List.toArray_replicate (α := α) n v).symm
+
+def replicate : MetaM Methods :=
+  mkPostMethods #[
+    ``Vector.replicate_eq_mk_replicate, ``List.replicate_toArray,
+
+    ``List.replicate_succ, ``List.replicate_zero
+  ]
+
 def extract : MetaM Methods :=
   mkPostMethods #[
     ``Vector.extract_mk, ``List.extract_toArray,
-    
+
     ``List.extract_eq_take_drop
   ] ∪ drop ∪ take ∪ SymSets.General.ground
 
@@ -687,9 +1513,37 @@ def size : MetaM Methods :=
    ``List.length_cons, ``List.length_nil
   ]
 
+def _root_.Lean.Expr.foldr? (e : Expr) : Option (List Expr) :=
+  match_expr e with
+  | Vector.foldr α β _ f init xs => .some [α, β, f, init, xs]
+  -- `start = xs.size` ∧ `stop = 0`
+  | Array.foldr α β f init xs start stop => .some [α, β, f, init, xs]
+  | List.foldr α β f init xs => .some [α, β, f, init, xs]
+  | _ => .none
+#check List.foldr_toArray
+/--
+TODO: We ignore start/stop on purpose for the time being.
+      `Sym` does not play nice with `List.foldr_toArray` and `List.foldr_toArray'` sometimes...
+
+      This is currently unprovable.
+-/
+def foldr_toArrayButSane : Sym.Simp.Simproc := fun e => do
+  let_expr Array.foldr α β f init xs _ _ := e | return .rfl
+  let .some ⟨_, xs⟩ := Collection.ofExpr xs | throwError m!"cannot foldr:\n{xs} in:\n{e}"
+  let e' ← Sym.shareCommonInc <| mkApp5 (.const ``List.foldr e.getAppFn.constLevels!) α β f init xs
+  return .step e' (←mkSorry (←mkEq e e') false)
+
+  -- let .some (elems, ⟨⟨_, k, .some sz⟩, listExpr⟩) ← sequenced xs | return .rfl
+  -- let szGround ← simpWithGround! sz
+  -- match Sym.getNatValue? szGround with
+  -- | .none => throwError m!"Not ground:\n{szGround} in:\n{e}"
+  -- | .some _ =>
+
+  --   let .some appendVecColl := appendListColl.setSize sz |>.cast xsC.type.k | unreachable!
+
 def foldr : MetaM Methods :=
   mkPostMethods #[
-    ``Vector.foldr_mk, ``List.foldr_toArray', ``List.foldr_toArray,
+    ``Vector.foldr_mk, ``foldr_toArrayButSane, -- ``List.foldr_toArray, ``List.foldr_toArray',
 
     ``List.foldr_cons, ``List.foldr_nil,
 
@@ -700,6 +1554,15 @@ def sum : MetaM Methods :=
   mkPostMethods #[
     ``Vector.sum_eq_foldr
   ] ∪ foldr
+
+def unwrap : Sym.Simp.Simproc := fun e ↦ do
+  let_expr Simp.clapwrap _ e := e | return .rfl
+  return .rfl (done := true)
+
+def unwrap_s : MetaM Methods :=
+  mkPreMethods #[
+    ``Clap.Compiler.SymSets.Vector.unwrap
+  ]
 
 def set_mk : Sym.Simp.Simproc := fun e => do
   let_expr Vector.set t sz xs i x h := e | return .rfl
@@ -719,8 +1582,94 @@ def set : MetaM Methods :=
   mkPostMethods #[
     ``Vector.set_mk
     -- ``List.set_toArray,
-    
+
     -- ``List.set_cons_succ, ``List.set_cons_zero,
+  ]
+
+def set_pre : MetaM Methods :=
+  mkPreMethods #[
+    ``Vector.set_mk
+    -- ``List.set_toArray,
+
+    -- ``List.set_cons_succ, ``List.set_cons_zero,
+  ]
+
+
+  -- let t ← Sym.inferType e
+  -- let_expr Vector t sz := t | return .rfl
+  -- unless e.isFVar do return .rfl
+  -- let sz' ← Sym.simpWithGround sz
+  -- match (sz'.getResultExpr sz).nat? with
+  -- | .none => throwError m!"{sz} does not simplify to ground.\nExpr:\n{e}"
+  -- | .some _n => let explodedVec ← (sequenceAsVecExpr e t (sz'.getResultExpr sz)).run'
+  --               trace[Clap.Compile.simp.proc.kaboom] m!"{who}"
+  --               -- trace[Clap.Compile.simp.proc.kaboom] m!"Exploding:\n{e}\n==>\n{explodedVec}"
+  --               return .step explodedVec (←mkSorry (←mkEq e explodedVec) false)
+
+-- private def explodeWrapper {α : Type} {k} (inner : Vector α k) (who : String := ""): Vector α k := inner
+
+-- private def unwrap : Sym.Simp.Simproc := fun e ↦ do
+--   let_expr Simp.clapwrap _ e := e | return .rfl
+--   return .rfl (done := true)
+
+-- def explode! : Sym.Simp.Simproc := fun e ↦ do
+--   let_expr explodeWrapper τ sz e who := e | return .rfl
+--   unless e.isFVar do return .rfl
+--   let sz' ← Sym.simpWithGround sz
+--   let sz' := sz'.getResultExpr sz
+--   match Sym.getNatValue? sz' with
+--   | .none => throwError m!"[unreachable]\n{sz} does not simplify to ground in:\n{e}"
+--   | .some _n => let explodedVec ← (sequenceAsVecExpr e τ sz').run'
+--                 trace[Clap.Compile.simp.proc.kaboom] m!"{who}"
+--                 -- trace[Clap.Compile.simp.proc.kaboom] m!"Exploding:\n{e}\n==>\n{explodedVec}"
+--                 return .step explodedVec (←mkSorry (←mkEq e explodedVec) false)
+
+
+-- private def wrappedInExplosives (τ sz who : Expr) : Sym.Simp.SimpM Expr := do
+--   let τu ← Sym.getLevelInType τ
+--   let vectorτ ← Sym.shareCommonInc <| mkApp2 (.const ``Vector [τu]) τ sz
+--   Sym.shareCommonInc <| mkApp4 (.const ``explodeWrapper [τu]) τ sz vectorτ who
+
+-- private def wrapInExplosives (τ sz who e : Expr) : Sym.Simp.SimpM Result := do
+--   let e' ← wrappedInExplosives τ sz who
+--   return .step e' (←mkSorry (←mkEq e e') false)
+
+-- def explode? : Sym.Simp.Simproc := fun e ↦ do
+--   if let .some [α, β, γ, xs, ys] := e.append?
+--   then
+--     let .some xs := Collection.elemsOfExpr xs | return .rfl
+--     let .some ys := Collection.elemsOfExpr ys | return .rfl
+--     return mkApp
+--   else
+--     return .rfl
+
+
+def processWrapped : Sym.Simp.Simproc := fun e ↦ do
+  let_expr Simp.clapwrap _ e := e | return .rfl
+  return .rfl (done := true)
+
+def wrapped : MetaM Methods :=
+  mkPreMethods #[``processWrapped]
+
+def unfold_generic_collection_functions_pre : MetaM Methods :=
+  mkPreMethods #[
+    -- `Clap.Compiler.SymSets.Vector.unfold_generic_mk_foldlM,
+    ``Clap.Compiler.SymSets.Vector.foldlM_stagger,
+    `Clap.Compiler.SymSets.Vector.getElem_mk,
+    `Clap.Compiler.SymSets.Vector.set_mk
+  ]
+
+def unfold_generic_collection_functions_post : MetaM Methods :=
+  mkPostMethods #[
+    -- `Clap.Compiler.SymSets.Vector.unfold_generic_mk_foldlM,
+    ``Clap.Compiler.SymSets.Vector.foldlM_stagger,
+    `Clap.Compiler.SymSets.Vector.getElem_mk,
+    `Clap.Compiler.SymSets.Vector.set_mk
+  ]
+
+def foldlM_stagger_post : MetaM Methods :=
+  mkPostMethods #[
+    ``Clap.Compiler.SymSets.Vector.foldlM_stagger,
   ]
 
 end Vector
@@ -748,16 +1697,219 @@ end
 
 end SymSets
 
-def compileJustSym (e : Expr) (simpset : Sym.Simp.Methods) : Sym.Simp.SimpM Expr := do
-  lambdaTelescope e fun args e ↦ do
-    let time ← IO.monoMsNow
-    let compiled ← Compiler.Simp.simplify (simpset) e -- ∪ (←SymSets.General.compilerSet)) e
-    -- logInfo m!"Compiled:\n{compiled}"
-    Dbg.timeSince time "Compilation took:"
-    Sym.mkLambdaFVarsS args compiled -- >>= (liftM ∘ PrettyPrinter.ppExpr)
+abbrev Simplifier := Expr → Sym.Simp.SimpM Expr
 
-def compileExampleJustSym (ex : Name) (simpset : Sym.Simp.Methods) : Sym.Simp.SimpM Expr := do
-  let e := ((←getEnv).find? ex).get!.value!
+/--
+- `a : Option α` = `⟨uα, α, a⟩`
+-/
+structure Action where
+  u : Level
+  α : Expr
+  a : Expr
+  deriving Repr
+
+def Action.simplifyUsing (a : Action) (simp : Simplifier) : Sym.Simp.SimpM Action :=
+  let ⟨u, α, a⟩ := a
+  simp a >>= (return ⟨u, α, ·⟩)
+
+/--
+- `f : α → Option β` = `⟨uα, uβ, α, β, f⟩`
+-/
+structure Cont where
+  u : Level
+  v : Level
+  α : Expr
+  β : Expr
+  f : Expr
+  deriving Repr
+
+/--
+- `Option.bind.{u, v} α β a f`
+-/
+structure Bind where
+  u  : Level
+  v  : Level
+  α  : Expr
+  β  : Expr
+  aₗ : Expr
+  aᵣ : Expr
+  deriving Repr
+
+def Bind.toExpr (bind : Bind) : Expr :=
+  let ⟨u, v, α, β, a, f⟩ := bind
+  mkApp4 (.const ``Option.bind [u, v]) α β a f
+
+def Bind.toCont (bind : Bind) : Cont :=
+  let ⟨u, v, α, β, _, f⟩ := bind
+  ⟨u, v, α, β, f⟩
+
+def Bind.explode (bind : Bind) : Action × Cont :=
+  let ⟨u, v, α, β, a, f⟩ := bind
+  (⟨u, α, a⟩, ⟨u, v, α, β, f⟩)
+
+/--
+NB: `Bind.bind` better be instantiating `Option`.
+-/
+private def _root_.Lean.Expr.matchBinds (e : Expr) : Sym.SymM (Option Bind) := do
+  match_expr e with
+  | Bind.bind _ _ α β a f => return .some ⟨←Sym.getLevelInType α, ←Sym.getLevelInType β, α, β, a, f⟩
+  | Option.bind   α β a f => return .some ⟨←Sym.getLevelInType α, ←Sym.getLevelInType β, α, β, a, f⟩
+  | _                     => return .none
+
+private def _root_.Lean.Expr.isUnital (e : Expr) : Bool :=
+  match_expr e with
+  | Unit  => true
+  | PUnit => true
+  | _     => false
+
+structure ActionWithResult where
+  action : Expr
+  result : Expr
+
+abbrev InProgressExpr := ActionWithResult ⊕ Expr
+
+def logRewrite (e e' : Expr) (decorate : String := "") : MessageData :=
+  m!"\n{e}\n={decorate}=>\n{e'}"
+
+-- def inlineFirst (e : Expr) : Expr :=
+--   match e.matchBindsEInfo with
+--   | .some (levels, #[α, β, a, f]) =>
+--     let tail := mkApp4 (.const ``Option.bind levels) α β a f
+--     _
+--   | _ => e
+
+
+-- def firstAction (e : Expr) : Expr × Option Expr :=
+--   go e
+--   where
+--     go (e : Expr) (rest : Option Expr) : Expr × Option Expr :=
+--     match e.matchBindsE with
+--     | .none => (e, rest)
+--     | .some (a, f) => let res := go a ()
+
+-- mutual
+
+-- private partial def down (reduce reduceOuter : Simplifier)
+--                          (stack : List InProgressExpr) (todo : Expr)
+--                          : Sym.Simp.SimpM Expr := do
+--   SymSets.General.inDebugOnly (do modifyDbgState fun σ ↦ {σ with numDown := σ.numDown + 1})
+--   -- See the docs of `unwrapped`
+--   -- let todo := unwrapped todo
+--   let .some ⟨_, _, _, β, _, _⟩ ← todo.matchBinds | return todo
+--   let binds := todo.sequenceBindsL -- do A; B; let x ← C; D; E ==> [A, B, C, D, E]
+--   logInfo m!"e: {todo}\nbinds:"
+--   let simpedBinds ← binds.mapM fun (action, τ) ↦ do
+--     -- let (simped, time) ← Dbg.timeS (reduce action)
+--     -- trace[Clap.Compile.down] logRewrite action simped
+--     -- SymSets.General.inDebugOnly do trace[Clap.Compile.dbg] m!"simp took {time}s"
+--     -- return (simped, τ)
+--     return (action, τ)
+--   let binds := SymSets.Vector.chainActions β simpedBinds
+--   logInfo m!"binds: {←binds}"
+--   binds
+
+--   -- if let .some ⟨_, _, _, _, a, f⟩ ← todo.matchBinds -- TODO(perf): Propagate the rest.
+--   -- then
+--   --   trace[Clap.Compile.down] m!"\npush [→]:\n{f}\ngo [↓]:\n{a}"
+--   --   down reduce reduceOuter (.inr f :: stack) a
+--   -- else
+--   --   let (simped, time) ← Dbg.timeS (reduce todo)
+--   --   inDebugOnly (do
+--   --     trace[Clap.Compile.dbg] m!"simp [↓] took {time}s"
+--   --     modifyDbgState fun σ ↦ {σ with cumulativeSimpTimeDown := σ.cumulativeSimpTimeDown + time}
+--   --   )
+--   --   if !Sym.isSameExpr simped todo
+--   --   then
+--   --     trace[Clap.Compile.simp] "[↓] {checkEmoji}\n{todo}\n==>\n{simped}"
+--   --     trace[Clap.Compile.down] "\ngo [↓]:\n{simped}"
+--   --     down reduce reduceOuter stack simped
+--   --   else
+--   --     trace[Clap.Compile.simp.fail] "[↓] {crossEmoji}\n{todo}"
+--   --     trace[Clap.Compile.down] "\ngo [↑]:\n{todo}"
+--   --     -- match ←isGroundTerm todo with
+--   --     -- | .some e => trace[Clap.Compile.simp.warnDownNotGround] "{stopEmoji} [↓] stopped:\n{e}"
+--   --     -- | .none => pure ()
+--   --     up reduce reduceOuter stack todo
+
+-- private partial def up (reduce reduceOuter : Simplifier)
+--                        (stack : List InProgressExpr) (done : Expr) : Sym.Simp.SimpM Expr := do
+--   SymSets.General.inDebugOnly (modifyDbgState fun σ ↦ {σ with numUp := σ.numUp + 1})
+--   match stack with
+--   | [] =>
+--     trace[Clap.Compile.up] "Done"
+--     return done
+--   | .inr e :: stack => do
+--     -- TODO: Bad idea to use the One! guy, need to eta-expand if need be if so...
+--     lambdaTelescope e fun arg body ↦ do
+--       let #[arg] := arg | unreachable!
+--       trace[Clap.Compile.up] "\npush [←]:\n{(done, arg)}\ngo [↓]:\n{body}"
+--       down reduce reduceOuter (.inl {action := done, result := arg} :: stack) body
+--   | .inl ⟨a, result⟩ :: stack => do
+--     let bind ← mkBindWith a result done
+--     let up := up reduce reduceOuter stack
+--     let lamArgT ← Sym.inferType result -- TODO(perf): Propagate universe/type info from `matchBinds`.
+--     if lamArgT.isUnital
+--     then trace[Clap.Compile.up] "\ngo [↑]:\n{bind}"
+--          up bind
+--     else trace[Clap.Compile.simp] "Binding value: {result} in {bind}"
+--          let (simped, time) ← Dbg.timeS (reduceOuter bind)
+--         --  let (simped, time) := (bind, 0)
+--          SymSets.General.inDebugOnly (do
+--            trace[Clap.Compile.dbg] m!"simp [↑] took {time}s"
+--            trace[Clap.Compile.dbg] m!"\n{bind}\n==>\n{simped}"
+--            modifyDbgState fun σ ↦ {σ with cumulativeSimpTimeUp := σ.cumulativeSimpTimeUp + time}
+--          )
+--          -- TODO(semantics): Ok we simped, so what?
+--          if !Sym.isSameExpr simped bind
+--          then trace[Clap.Compile.simp] "[↑] {checkEmoji}\n{bind}\n==>\n{simped}"
+--          else trace[Clap.Compile.simp.fail] "[↑] {crossEmoji}\n{bind}"
+--          trace[Clap.Compile.up] "\ngo [↑]:\n{simped}"
+--          up simped
+--   where mkBindWith (a result k : Expr) : Sym.Simp.SimpM Expr := do
+--     -- TODO(perf): Propagate universe/type info from `matchBinds`.
+--     -- logInfo m!"a: {a}\nresult: {result}\nk: {k}"
+--     let α ← result.fvarId!.getType
+--     let u ← Sym.getLevelInType α
+--     let β ← Sym.inferType k
+--     let_expr Option t' := β | throwError m!"Body return not in `Option. Shouldn't be happening."
+--     let v ← Sym.getLevelInType t'
+--     let f ← Sym.shareCommonInc (←Sym.mkLambdaFVarsS #[result] k)
+--     Sym.shareCommonInc <| mkApp4 (.const ``Option.bind [u, v]) α β a f
+
+-- end
+
+-- def compile (e : Expr) (simpset : Sym.Simp.Methods := default) : Sym.Simp.SimpM Expr := do
+--   let simpset! ← SymSets.Vector.monads! ∪ return simpset
+--   let e ← Compiler.Simp.preprocessExpr e
+--   lambdaTelescope e fun args e ↦ do
+--     let compiled ← down
+--       (reduce      := Compiler.Simp.simplify simpset!)
+--       (reduceOuter := Compiler.Simp.simplify simpset!)
+--       -- (reduceOuter := Compiler.Simp.simplify simpset)
+--       (stack       := [])
+--       (todo        := e)
+--     SymSets.General.inDebugOnly do trace[Clap.Compile.dbg] m!"σ: {←(←getDbgState).pretty}"
+--     Sym.shareCommonInc (←mkLambdaFVars args compiled)
+
+-- def compileExample (ex : Name) (simpset : Sym.Simp.Methods := default) (args : Array Expr := #[]) : Sym.Simp.SimpM Expr := do
+--   -- withTraceNode `Clap.Compile.simp.proc (fun e ↦ return m!"") do
+--   let e := ((←getEnv).find? ex).get!.value!.beta args
+--   compile e simpset
+
+def compileJustSym (e : Expr) (simpset : Sym.Simp.Methods) : Sym.Simp.SimpM Expr := do
+  let e ← Compiler.Simp.preprocessExpr e
+  let res ← lambdaTelescope e fun args e ↦ do
+    let time ← IO.monoMsNow
+    let compiled ← Compiler.Simp.simplify simpset e
+    Dbg.timeSince time "Compilation took:"
+    let σ ← getDbgState
+    logInfo m!"{←σ.pretty}"
+    Sym.mkLambdaFVarsS args compiled
+  Sym.shareCommonInc res
+
+def compileExampleJustSym (ex : Name) (simpset : Sym.Simp.Methods) (args : Array Expr := #[]) : Sym.Simp.SimpM Expr := do
+  -- withTraceNode `Clap.Compile.simp.proc (fun e ↦ return m!"") do
+  let e := ((←getEnv).find? ex).get!.value!.beta args
   compileJustSym e simpset
 
 open SymSets in
@@ -766,201 +1918,1080 @@ elab "compile_just_sym" "[" simps:ident,* "]" : tactic => do
   let methods ← simps.mapM (liftM ∘ Simp.API.getMethodsM)
   let methods ← liftM <| methods.foldl (fun method acc ↦ method ∪ acc) (pure {})
   Tactic.liftMetaTactic1 fun mvarId => Sym.SymM.run do
-    let mvarId ← Sym.preprocessMVar mvarId    
+    let mvarId ← Sym.preprocessMVar mvarId
     let time ← IO.monoMsNow
     let res ← (← Sym.simpGoal mvarId methods).toOption
     logInfo m!"compile_just_sym took {Dbg.timeInSecondsOfMs time (←IO.monoMsNow)}s"
     return res
 
+def reportAttempt : Sym.Simp.Simproc := fun e ↦ do
+  discard bump
+  return .rfl
+
+def rewriteReport : Sym.Simp.Simproc := fun e ↦ do
+  let stuff ← Sym.Simp.mkTheoremFromDecl `Clap.Compiler.ExampruSym.a
+  let res ← stuff.rewrite e
+  match res with
+  | .rfl .. => return res
+  | .step .. =>
+    logInfo m!"Did the rewrite"
+    return res
+
+-- bind (bind (bind x fun y₂ ↦ g (fun y₄ ↦ y₄)) fun y₃ ↦ g') fun y ↦ bind x₁ fun y₁ ↦ bind x₂ g''
+-- [(x, fun y ↦ x), ..., ..., ] -- List.cons
+/-
+do
+  do
+    do
+      x
+      do
+-/
+
 elab "sym_simp" "[" declNames:ident,* "]" : tactic => do
-  let rewrite ← Sym.mkSimprocFor (← declNames.getElems.mapM fun s => realizeGlobalConstNoOverload s.raw) Sym.Simp.dischargeNone
+  resetCounter
+  -- let rewrite ← Sym.mkSimprocFor (← declNames.getElems.mapM fun s => realizeGlobalConstNoOverload s.raw) Sym.Simp.dischargeNone
+  -- let methods : Sym.Simp.Methods := {
+  --   pre  := fun _ ↦ return .rfl
+  --   post := reportAttempt >> rewriteReport
+  -- }
   let methods : Sym.Simp.Methods := {
     pre  := fun _ ↦ return .rfl
-    post := rewrite
+    post := reportAttempt >> Clap.Compiler.SymSets.General.betaReduce >> rewriteReport
   }
   Tactic.liftMetaTactic1 fun mvarId => Sym.SymM.run do
     let mvarId ← Sym.preprocessMVar mvarId
     let time ← IO.monoMsNow
     let res ← (← Sym.simpGoal mvarId methods).toOption
     logInfo m!"sym_simp took {Dbg.timeInSecondsOfMs time (←IO.monoMsNow)}s"
+    logInfo m!"this many times: {←getCounter}"
     return res
 
 def eq0 (e : Nat) : Option Unit := .some ()
 
-def spoon (m : Sym.Simp.SimpM Expr) : MetaM Unit := do
-  let compiled ← m.run' {} |>.run
-  logInfo m!"Compiled:\n{compiled}"
-  -- (m.run' {} |>.run) >>= PrettyPrinter.ppExpr
+opaque f : Option Unit
+
+def tt : Option Unit :=
+  Option.bind (eq0 0) fun _ ↦
+  Option.bind
+    (/- _ ↦-/Option.bind f
+     fun _ ↦ Option.bind (.some 4)
+     fun x ↦ Option.bind (.some <| x + 1)
+     fun y ↦ .some <| y + x + x + 2) fun y ↦
+  eq0 y
+
+/-
+ind_assoc:
+(eq0 0).bind fun a =>
+  f.bind fun a => (some 4).bind fun a => (some (a + 1)).bind fun y => (some (y + 2)).bind fun y => eq0 y
+
+compile:
+(eq0 0).bind fun x =>
+  f.bind fun a => (some 4).bind fun a => (some (a + 1)).bind fun a => (some (a + 2)).bind fun a => eq0 a
+-/
+
+def tt' : Option Unit :=
+  Option.bind (eq0 0) fun _ ↦
+  Option.bind f fun _ ↦
+  Option.bind (.some 4) fun x ↦
+  Option.bind (.some <| x + 1) fun y ↦
+  Option.bind (.some <| y + 2) fun y ↦
+  eq0 y
+
+-- example : tt = tt' := by
+--   unfold tt
+--   compile_just_sym [SymSets.Vector.bindMyAssoc_set]
+--   simp only [←Option.bind_eq_bind]
+--   simp only [bind_assoc]
+--   unfold tt'
+
+--   rw [Option.bind_assoc]
+--   rw [Option.bind_assoc]
+--   rw [Option.bind_some]
+--   rw [Option.bind_some]
+--   rw [Option.bind_some]
+--   rw [Option.bind_some]
+--   rw [Option.bind_some]
+--   rw [Option.bind_some]
+--   rfl
+--   -- compile_just_sym [SymSets.Vector.bindMyAssoc_set]
+
+def ppMonad (e : Expr) : MetaM Expr := do
+  let pretty ← Sym.simp e (←Clap.Compiler.SymSets.General.compilerBindEqBind) |>.run
+  return pretty.getResultExpr e
+
+/-- a.k.a tablespoon -/
+def liftExpr (m : Sym.Simp.SimpM Expr) : MetaM Expr := do
+  m.run' {} |>.run
+
+def spoon (m : Sym.Simp.SimpM Expr) (pretty := true) : MetaM Unit := do
+  let compiled ← liftExpr m
+  if pretty then
+    let pretty ← ppMonad compiled
+    logInfo m!"Compiled:\n{pretty}"
+  else
+    logInfo m!"Compiled:\n{compiled}"
+
+def x :=
+  let x := 42
+  x
+
+#eval ToExpr.toExpr x
+#check OfNat.ofNat
+run_meta do
+  let env ← getEnv
+  let c := env.find? ``x |>.get!
+  logInfo m!"c: {repr c.value!}"
+
+#eval spoon do
+  let env ← getEnv
+  let impl := env.find? ``x |>.get!.value!
+  let preprocessed ← Compiler.Simp.preprocessExpr impl
+  logInfo m!"old:\n{impl}\nnew:\n{preprocessed}"
+  return preprocessed
+
+
+  -- -- (m.run' {} |>.run) >>= PrettyPrinter.ppExpr
+
+open Sym in
+/--
+Applies hash-consing to `e`. Recall that all expressions in a `grind` goal have
+been hash-consed. We perform this step before we internalize expressions.
+-/
+def shareCommon (e : Expr) : Sym.SymM Expr := do
+  let share ← modifyGet fun s => (s.share, { s with share := {} })
+  let (e, share) := shareCommonAlpha e share
+  modify fun s => { s with share }
+  return e
+
+open Sym.Simp in
+public def simpLambda' (simpBody : Simproc) (e : Expr) : Sym.Simp.SimpM Result := do
+  lambdaTelescope e fun xs b => withFreshTransientCache do
+    main xs (← shareCommon b)
+where
+  main (xs : Array Expr) (b : Expr) : Sym.Simp.SimpM Result := do
+    let σ ← get
+    let σ := σ.transientCache
+    logInfo m!"START"
+    for (k, v) in σ do
+      logInfo m!"{k.expr} → {v.getResultExpr default}"
+    logInfo m!"THE END"
+    -- Propagate `cd` from the body: in another context the body might simplify differently.
+    match (← simpBody b) with
+    | .rfl _ cd => return mkRflResultCD cd
+    | .step b' h _ cd =>
+      let h ← mkLambdaFVars xs h
+      let e' ← shareCommon (← mkLambdaFVars xs b')
+      return .step e' (←mkSorry (←mkEq e e') false) (contextDependent := cd)
+
+-- def f := fun x : Nat => (x, fun x₁ : Nat => (x₁, fun x₂ : Nat => x₂))
+
+-- -- `def f := fun x : Nat ↦ fun y : Nat ↦ ...`
+-- #check Sym.AlphaKey
+-- def inst : Hashable Nat := ⟨fun _ ↦ 0⟩
+-- #check Prod.mk
+-- def abc : Sym.Simp.SimpM Unit := do
+--   -- let m : @Std.HashMap Nat Nat inferInstance inst :=
+--   --   @Std.HashMap.ofArray _ _ _ inst #[(0, 1), (1, 2), (2, 3)]
+--   -- for (k, v) in m do
+--   --   logInfo m!"{k} → {v}"
+--   let env ← getEnv
+--   let .some stuff := env.find? ``Clap.Compiler.f | unreachable!
+--   let val := stuff.value!
+--   let σ ← get
+--   let σ := σ.transientCache
+--   for (k, v) in σ do
+--     logInfo m!"{k.expr} → {v.getResultExpr default}"
+--   return ()
+
+-- #eval abc.run' {} |>.run
+
+-- #exit
+  -- let σshare₁ := σ.share
+  -- for key in σshare₁.set do
+  --   logInfo m!"{key.expr}"
+  -- logInfo m!"______________________"
+  -- let impl ← Sym.shareCommon val
+  -- logInfo m!"impl: {impl}"
+  -- let σ₂ ← get
+  -- let σshare₂ := σ₂.share
+  -- let cache₂ := σshare₂.set.toList
+  -- let cache₂sorted := cache₂.mergeSort (le := fun e₁ e₂ ↦ e₁.expr.sizeWithoutSharing ≤ e₂.expr.sizeWithoutSharing)
+  -- for key in cache₂sorted.zipIdx do
+  --   let val := key.1.expr
+  --   let_expr Prod.mk _ _ fst snd := val | continue
+  --   let res := cache₂sorted.find? fun e ↦ Sym.isSameExpr e.expr snd
+  --   logInfo m!"res: {Sym.AlphaKey.expr <$> res}"
+  --   if σshare₁.set.contains key.1
+  --   then logInfo m!"{checkEmoji}[{key.2}] {key.1.expr}"
+  --   else logInfo m!"{crossEmoji}[{key.2}] {key.1.expr}"
+  --   logInfo m!"fst: {fst} snd: {snd}"
+  -- logInfo m!"first: {σshare₁.set.toList.length}"
+  -- logInfo m!"second: {σshare₂.set.toList.length}"
+  -- logInfo m!"{←PrettyPrinter.ppExpr (cache₂sorted[28]'sorry).expr}"
+
+-- #eval! abc.run
 
 namespace ExampruSym
 
+namespace NewTraversal
 open SymSets Monad General Vector
 
-set_option trace.Clap.Compile true
+opaque F : ℕ → Option ℕ
+opaque G : ℕ → Option ℕ
+opaque H : ℕ → Option ℕ
 
-def ex₀ : Option Unit := do
-  eq0 0
-  eq0 1
-  let _res ← ([0, 1].foldlM (init := ()) fun _ _ ↦ eq0 2)
-  eq0 3
-  return ()
+def exex : Option Unit :=
+  Option.bind (eq0 4) fun _ : Unit ↦
+    Option.bind
+      ((Option.bind
+         (Option.bind
+           (Option.bind
+             (F 2) fun x ↦
+            Option.bind (F 3) fun y ↦ G (x + y))
+           fun x ↦ H x))
+         fun x ↦ F x) fun x ↦
+      F x
 
-/--
-info: Compiled:
-(eq0 0).bind fun x =>
-(eq0 1).bind fun x =>
-(eq0 2).bind fun y =>
-(eq0 2).bind fun _res =>
-(eq0 3).bind fun x => some PUnit.unit
--/
-#guard_msgs(info, whitespace := lax, drop warning) in
-#eval spoon <| do compileExampleJustSym ``ex₀ (←(foldlM ∪ compilerSet_old'))
+#print exex
 
-def ex₁ (_vec : Vector Nat 3) : Option Unit := do
-  eq0 #v[4, 5][0]
+def testInnerReturn : Option Unit := do
+  let x ← F 1
+  let y ← F (←(fun (x: ℕ) => do
+    return x) 3)
+  let z ← F 3
+  pure ()
 
-/--
-info: Compiled:
-fun _vec => eq0 4
--/
-#guard_msgs(info, whitespace := lax, drop warning) in
-#eval spoon <| do compileExampleJustSym ``ex₁ (←getElem)
+-- set_option trace.Clap.Compile true in
+-- set_option Clap.traversalDbg true in
+-- set_option trace.Clap.Compile.dbg true in
+-- #eval spoon <| do
+--   let e ← compileExample ``testInnerReturn (←(mapM_singlePass_pre))
+--   -- Pretty print (i.e. go back to `Bind.bind`)
+--   return (←Sym.simp e (←compilerBindEqBind)).getResultExpr e
 
-def ex₂ (vec : Vector Nat 3) : Option Unit := do
-  let x := (vec ++ vec)[0] -- `GetElem (Vector _ (3 + 3))`
+
+def exex' : Option Unit := do
+  let z ← F 2
+  let x ← H 4
+  let y ← (do let x ← G (x + z); let y ← G x; H (x + z))
+  H y
+
+def exex'' : Option Unit := do
+  let z ← F 2
+  let x ← #v[1, 2].mapM (fun _ ↦ pure 4)
+  let y ← (do let x ← G x[1]; let y ← G x; H (x + z))
+  H y
+
+#check @Option.bind_assoc
+
+-- set_option trace.Clap.Compile true in
+-- set_option Clap.traversalDbg true in
+-- set_option trace.Clap.Compile.dbg true in
+-- #eval spoon <| do
+--   let e ← compileExample ``exex'' (←(mapM_singlePass_pre))
+--   -- Pretty print (i.e. go back to `Bind.bind`)
+--   return (←Sym.simp e (←compilerBindEqBind)).getResultExpr e
+
+
+def eq0 (e : Nat) : Option Unit := .some ()
+
+def ex₈ (n : ℕ) (vec : Vector Nat n) : Option Unit := do
+  let x ← (do let _ ← eq0 2; let X ← vec.mapM (fun x ↦ (eq0 (x + 42) : Option _)); return 4)
   eq0 x
-/--
-info: Compiled:
-fun vec => eq0 vec[0]
+
+opaque share : Nat → Option Nat
+
+def ex₉ {n : Nat} (vec : Vector Nat n) : Option Unit := do
+  let x ← (do let _ ← eq0 2; let x ← vec.mapM (fun x ↦ (share (x + 42) : Option _)); return x)
+  let _ ← x.mapM eq0
+
+set_option maxRecDepth 1024 in
+set_option trace.Clap.Compile.dbg true in
+set_option Clap.traversalDbg true in
+set_option trace.Clap.Compile true in
+#eval do
+  let (e, time) ← Dbg.timeS <| compileExampleJustSym (args := #[toExpr 10]) ``ex₉
+    (←(
+      mapM ∪
+      getElem ∪
+      append ∪
+      explode -- ∪ monads -- ∪ zeta ∪ monads ∪ explode
+    ∪ compilerAssoc
+    -- ∪ bindMyAssoc_set
+    ∪ monads
+    -- mapM_alt
+    )) |>.run' {} |>.run
+  logInfo m!"time: {time}"
+  -- let e' := Sym.simp e {}
+  let e' := Sym.simp e (←compilerBindEqBind)
+  let e' ← e'.run
+
+  logInfo m!"e: {e'.getResultExpr e}"
+  -- logInfo m!"{←(getAndResetDbgState)}"
+
+-- set_option Clap.traversalDbg true
+-- set_option trace.Clap.Compile.dbg false
+-- def bench : MetaM Unit := do
+--   let simpset := (←(SymSets.Vector.wrapped ∪ mapM_mk ∪ explode ∪ compilerAssoc))
+--   -- let simpset := (←(mapM_singlePass ∪ zeta ∪ explode))
+--   let inputSizes := (Array.range 2).map (10 * 2^·)
+--   let timings ← inputSizes.mapM fun inputSize ↦ do
+--     let res ← Dbg.timeS <| (compileExample ``ex₉ simpset (args := #[mkNatLit inputSize])).run' {} |>.run
+--     let σ ← getAndResetDbgState
+--     return (inputSize, res, σ)
+--   for (n, (compiled, time), dbgState) in timings do
+--     logInfo m!"ex₈[{n}] took {time}s"
+--     logInfo m!"dbg: {←dbgState.pretty}"
+
+--     logInfo m!"{←ppMonad compiled}"
+
+-- #eval bench
+
+opaque A : Nat → Option Nat
+opaque B : Nat → Option Nat
+opaque C : Nat → Option Nat
+opaque D : Nat → Option Nat
+opaque E : Nat → Option Nat
+
+def e? (vec : Vector Nat 4) : Option Unit := do
+  let _ ← A 1
+  let z ← B 2
+  let x ←
+    (do let _ ← F 4
+        let x ←
+          (do
+            let _ ← C 42; let w ← D z; let _ ← D 42
+            let y ← (do let x ← D 9; let y ← H 99; return x + y)
+            E (z + w)
+          )
+        H x)
+  F x
+
+def eboom (vec : Vector Nat 4) : Option Unit := do
+  let x ←
+    (do
+      let w ← A 0
+      let x ←
+        (do let y ← do
+            let z ← B 1
+            let res ←
+              (do let w ← C 2
+                  D 5)
+            E res)
+      F (w + x)
+    )
+  discard (G x)
+
+def eboom' (vec : Vector Nat 4) : Option Unit := do
+  let x ←
+    (do
+      let w ← A 0
+      let x ←
+        (do let y ← do
+            let z ← B 1
+            let w ← (do let y ← do
+                        let z ← B 1
+                        let res ←
+                          (do let w ← C 2; D 5)
+                        E res)
+            let res ←
+              (do let w ← C 2; D 5)
+            E res)
+      F (w + x)
+    )
+  discard (G x)
+
+def assocPre : MetaM Sym.Simp.Methods :=
+  mkPreMethods #[
+    ``bind_assoc
+  ]
+
+def assocPost : MetaM Sym.Simp.Methods :=
+  mkPostMethods #[
+    ``bind_assoc
+  ]
+
+partial def _root_.Lean.Expr.sequenceBindsLM (e : Expr) : Sym.Simp.SimpM (Array (Expr × Expr)) :=
+  go #[e] #[]
+where
+  go (todo : Array Expr) (done : Array (Expr × Expr)) : Sym.Simp.SimpM (Array (Expr × Expr)) := do
+    match todo.back? with
+    | .none => return done
+    | .some e =>
+      let todo := todo.pop
+      match e.matchBindsE with
+      | .some (action, func) =>
+        match action.matchBindsE with
+        | .some (b, g) =>
+          go (todo.append #[func, g, b]) done
+        | _ =>
+          go (todo.push func) (done.push (action, default))
+      | _ =>
+        match e with
+        | .lam _ dom body _ =>
+          let done := done.modify done.size.pred fun (a, _) ↦ (a, dom)
+          go (todo.push body) done
+        | _ =>
+          go todo (done.push (e, default))
+
+partial def _root_.Lean.Expr.sequenceBindsLMSansType (e : Expr) : Sym.Simp.SimpM (Array Expr) :=
+  go #[e] #[]
+where
+  go (todo : Array Expr) (done : Array Expr) : Sym.Simp.SimpM (Array Expr) := do
+    match todo.back? with
+    | .none => return done
+    | .some e =>
+      let todo := todo.pop
+      match e.matchBindsE with
+      | .some (action, func) =>
+        match action.matchBindsE with
+        | .some (b, g) =>
+          go (todo.append #[func, g, b]) done
+        | _ =>
+          go (todo.push func) (done.push action)
+      | _ =>
+        match e with
+        | .lam _ _ body _ =>
+          go (todo.push body) done
+        | _ =>
+          go todo (done.push e)
+
+-- partial def _root_.Lean.Expr.sequenceBindsLM (e : Expr) : Sym.Simp.SimpM (Array (Expr × Expr)) :=
+
+opaque a : Option Unit
+opaque b : Option Unit
+opaque c : Option Unit
+opaque d : Option Unit
+opaque e : Option Unit
+
+def xb : Option Unit := do
+  a
+  let x ← (do a; b)
+  c
+  d
+  e
+
+example : xb = bind a (fun _ ↦ (bind (bind a fun _ ↦ b) fun _ ↦ bind c fun _ ↦ bind d fun _ ↦ e)) := by
+  rfl
+-- fun a ↦ fun b ↦ body
+-- telescope args = [a, b], body = body
+
+-- partial def _root_.Lean.Expr.sequenceBindsLButCorrect (e : Expr) : Sym.Simp.SimpM (Array Expr) := do
+--   match e.matchBindsE with
+--   | .some (a, .lam _ dom body _) =>
+--     let a' ← sequenceBindsLButCorrect a
+--     _
+--   | .none => return #[]
+--   | _ => _
+
+-- partial def _root_.Lean.Expr.sequenceBindsStrictLeft (e : Expr) : Sym.Simp.SimpM (Array (Expr × Expr)) :=
+--   go #[e] #[]
+-- where
+--   go (todo : Array Expr) (done : Array (Expr × Expr)) : Sym.Simp.SimpM (Array (Expr × Expr)) := do
+--     match todo.back? with
+--     | .none => return done
+--     | .some e =>
+--       let todo := todo.pop
+--       match e.matchBindsE with
+--       | .some (action, func) =>
+--         match action.matchBindsE with
+--         | .some (b, g) =>
+--           go (todo.append #[func, g, b]) done
+--         | _ =>
+--           go (todo.push func) (done.push (action, default))
+--       | _ =>
+--         match e with
+--         | .lam _ dom body _ =>
+--           -- TODO cover case of passing a lambda directly into sequenceBindsL
+--           -- `.lam x q(Nat) q(True) default` yields `(q(True), default)`, that's fine vOv
+--           let done := done.modify done.size.pred fun (a, _) ↦ (a, dom)
+--           go (todo.push body) done
+--         | _ =>
+--           go todo (done.push (e, default))
+
+-- def tryThisForSize : Sym.Simp.Simproc := fun e ↦ do
+--   let .some (_, #[_, β, _, _]) := e.matchBindsEInfo | return .rfl
+--   let seq ← e.sequenceBindsLM
+--   let binds ← SymSets.Vector.chainActions β seq
+--   let e' ← Sym.shareCommon binds
+--   logInfo m!"\n{e}\n==>\n{e'}"
+--   return .step e' (←mkSorry (←mkEq e e') false) (done := true)
+
+-- /-
+--     B
+--   B   fun ...
+-- A   fun ...
+-- -/
+-- def tryThatForSize : Sym.Simp.Simproc := fun e ↦ do
+--   let .some (_, #[_, outputτ, a, _]) := e.matchBindsEInfo | return .rfl
+--   let .some (_, #[_, _, _, _])       := a.matchBindsEInfo | return .rfl
+--   recordRuleDbg "tryThatForSize"
+--   let actionSequence ← e.sequenceBindsLM
+--   trace[Clap.Compile.dbg]
+--     m!"Action Sequence: {actionSequence}"
+--   let flatBind ← Sym.shareCommonInc (←SymSets.Vector.chainActionsInferType <| actionSequence.map Prod.fst)
+--   trace[Clap.Compile.dbg]
+--     m!"Flat Bind: {flatBind}"
+--   trace[Clap.Compile.dbg]
+--     m!"T: {←Sym.inferType flatBind}"
+
+  -- return .step flatBind (←mkSorry (←mkEq e flatBind) false)
+
+-- def spinalSurgeryStrictLeft_pre : MetaM Sym.Simp.Methods :=
+--   mkPreMethods #[
+--     ``tryThatForSize
+--   ]
+
+-- def spinalSurgery_pre : MetaM Sym.Simp.Methods :=
+--   mkPreMethods #[
+--     ``tryThisForSize
+--   ]
+
+set_option trace.Clap.Compile.dbg true
+set_option Clap.traversalDbg true
+set_option trace.Clap.Compile true
+#eval do
+  resetDbgState
+
+  let spinalSurgery ← compilerAssoc
+  -- let spinalSurgery ← spinalSurgery_pre
+  -- let spinalSurgery ← spinalSurgeryStrictLeft_pre
+
+  let (e, time) ←
+    Dbg.timeS <| compileExampleJustSym ``eboom spinalSurgery |>.run' {} |>.run
+
+  logInfo m!"time: {time}"
+  -- let e' := Sym.simp e {}
+  let e' := Sym.simp e (←compilerBindEqBind)
+  let e' ← e'.run
+
+  logInfo m!"e: {e'.getResultExpr e}"
+  let σ ← getAndResetDbgState
+  logInfo m!"{←σ.pretty}"
+
+-- #eval ExampruSym.runTest ``eboom
+
+#check bind_assoc
+/-
+            >>= h
+        >>=
+(x >>= f)  g
+becomes
+
+            >>= h
+        >>=
+(x >>= (λ x1, f x1))  (λ x2, g x2)
+
+
+
+  >>=
+x     λ x1
+        >>=
+    (f x1)  λ x2
+              >>=
+          (g x2)  h
+
+     >>=
+ >>=     g
+x   λ a
+
+any unbound bvars in the tree will have been converted to fvars by lambda telescoping as we get here
+
 -/
-#guard_msgs(info, whitespace := lax, drop warning) in
-#eval spoon <| do compileExampleJustSym ``ex₂ (←(getElem ∪ append ∪ zeta ∪ explode))
 
-def ex₃ (vec : Vector Nat 200) : Option Unit := do
-  let x := vec.map (·+1)
-  eq0 x[0]
+namespace Dom
+
+/-allowed patterns:
+      >>=
+   >>=     g
+  x   f
+
+    >>=
+  x    λ x
+        >>=
+      f x  g x
+-/
+
+def get_left_bind (expr: Expr): Option ((Expr × Expr × Expr) × (Expr × Expr × Expr)) := do
+  let_expr Option.bind midType outputType mid f2 := expr | .none
+  let_expr Option.bind inputType midType' input f1 := mid | .none
+  assert! midType == midType'
+  return ((inputType, midType, outputType), (input, f1, f2))
+
+def flattenBinds : Sym.Simp.Simproc := fun expr ↦ do
+  let Option.some outerBind := ←expr.matchBinds | return .rfl
+  let Option.some innerBind := ←(outerBind.aₗ).matchBinds | return .rfl
+  recordRuleDbg "Dom flatten"
+
+  let ((inputType, midType, outputType), (input, f1, f2)) :=
+    ((
+      innerBind.α,
+      innerBind.β,
+      outerBind.β
+    ),
+    (
+      innerBind.aₗ,
+      innerBind.aᵣ,
+      outerBind.aᵣ
+    ))
+
+  let func :=
+    Expr.lam
+      `x
+      inputType
+      (
+        mkApp4
+          (.const ``Option.bind [←Sym.getLevelInType midType, ←Sym.getLevelInType outputType])
+          midType
+          outputType
+          (f1.beta #[.bvar 0])
+          f2
+      )
+      .default
+
+  let bind :=
+    mkApp4
+      (.const ``Option.bind [←Sym.getLevelInType inputType, ←Sym.getLevelInType outputType])
+      inputType
+      outputType
+      input
+      func
+
+  let bind ← shareCommon bind
+
+  trace[Clap.Compile.simp.proc.flattenBinds]
+    m!"func: {func}\nbind: {bind}"
+
+  trace[Clap.Compile.simp.proc.flattenBinds]
+    logRewrite expr bind
+
+  return .step bind (←mkSorry (←mkEq expr bind) false)
+
+-- partial def flattenBinds' : Sym.Simp.Simproc := fun e ↦ do
+--   let Option.some outerBind := ←e.matchBinds | return .rfl
+--   let Option.some innerBind := ←(outerBind.aₗ).matchBinds | return .rfl
+
+--   let rec go (e : Expr) (level : ℕ) : Expr :=
+--     if let .some (a, f) := e.matchBindsE
+--     then
+--       let left := go a level
+--       let right := go a level.succ
+--       _
+
+--     else _
+
+--   _
+
+-- def flattenBinds_pre' : MetaM Sym.Simp.Methods :=
+--   mkPreMethods #[
+--     ``flattenBinds'
+--   ]
+
+def flattenBinds_pre : MetaM Sym.Simp.Methods :=
+  mkPreMethods #[
+    ``flattenBinds
+  ]
+
+-- /-
+-- TODO this is currently extermely specialised and not correct in unhandled cases
+-- needs to also substitute into actions
+-- could do with perhaps calling the substitution function directly rather than beta reducing?
+-- -/
+-- def applyMany (body: Expr) (args: List (Expr × Expr)) : Sym.SymM Expr := do
+--   let mut args := args
+--   for ((value, type), idx) in args.zipIdx do
+--     let (values, types) := args.unzip
+--     let value ← substitute_unbound_bvars
+--       value
+--       (values.take idx).toArray
+--       (types.take idx)
+--     let type ← substitute_unbound_bvars
+--       type
+--       (values.take idx).toArray
+--       (types.take idx)
+--     args := args.set idx (value, type)
+--   let (values, types) := args.unzip
+--   substitute_unbound_bvars body values.toArray types
+
+-- def bindPureMany_pre : MetaM Sym.Simp.Methods :=
+--   mkPreMethods #[
+--     ``pureBindMany
+--   ]
+
+-- def bindPureMany_post : MetaM Sym.Simp.Methods :=
+--   mkPostMethods #[
+--     ``pureBindMany
+--   ]
+#check Array.foldl
+
+-- /--
+--   consilium magnum - grand plan
+--   ire - go
+--   planus est - is flat
+-- -/
+-- partial def consiliumMagnum' (simpset : Sym.Simp.Methods) (e : Expr) (Γ : Std.HashSet Expr := {}) (dbg : Nat := 42) : Sym.Simp.SimpM Expr := do
+--   if dbg == 0 then return e
+--   let ire (e : Expr) (Γ : Std.HashSet Expr) := consiliumMagnum' simpset e Γ dbg.pred
+--   let simp (e : Expr) : Sym.Simp.SimpM Sym.Simp.Result := do
+--     let e' ← Sym.simp e simpset
+--     match e' with
+--     | .rfl .. => return e'
+--     | .step e' prf done ctxDep =>
+--       return .step (Simp.unwrapped e') prf done ctxDep
+--   match e.matchBindsEInfo with
+--   | .some (usᵣ, #[αᵣ, βᵣ, aᵣ, fᵣ]) =>
+--     if Γ.contains aᵣ
+--     then
+--       trace[Clap.Compile.consiliumMagnum]
+--         m!"Skip:\n{aᵣ}"
+--       ire fᵣ Γ
+--     else
+--       match aᵣ.matchBindsEInfo with
+--       | .some (wsₗ, #[αₗ, βₗ, aₗ, gₗ]) =>
+--         let e' ← planusEst e
+--         let e' ← chainActionsInferType e'
+--         trace[Clap.Compile.consiliumMagnum]
+--           m!"Flatten:\n{e}\n==>\n{e'}"
+--         ire e' Γ
+--       | _ =>
+--         -- TODO: Structure this better  
+--         let ωₗ ← simp aᵣ
+--         match ωₗ with
+--         | .rfl .. =>
+--           let Γ := Γ.insert aᵣ
+--           /-
+--             TODO: Using `pureBindMany` here would be ideal, but the intermediate `some`s
+--             need simping apriori.
+--           -/
+--           match ←bindPureMany e with
+--           | .step e' ..  =>
+--             trace[Clap.Compile.consiliumMagnum]
+--               m!"Feedforward:\n{e}\n==>\n{e'}"
+--             ire e' Γ
+--           | .rfl .. =>
+--             ire e Γ
+--         | .step ωₗ .. =>
+--           trace[Clap.Compile.consiliumMagnum]
+--             m!"Focus:\n{aᵣ}\nin:\n{e}\n==>\n{ωₗ}"
+--           let e' ← Sym.shareCommonInc <| mkApp4 (.const ``Option.bind usᵣ) αᵣ βᵣ ωₗ fᵣ
+--           ire e' Γ
+--   | _ =>
+--     let e' ← simp e
+--     let e' := e'.getResultExpr e
+--     trace[Clap.Compile.consiliumMagnum]
+--       m!"Simplify:\n{e}\n==>\n{e'}"
+--     if Sym.isSameExpr e e' then return e
+--     ire e' Γ
+
+-- def compilaCumStrategiaMagna' (e : Expr) (simpset : Sym.Simp.Methods) : Sym.Simp.SimpM Expr := do
+--   let e ← Compiler.Simp.preprocessExpr e
+--   let res ← lambdaTelescope e fun args e ↦ do
+--     let time ← IO.monoMsNow
+--     let compiled ← consiliumMagnum' simpset e
+--     Dbg.timeSince time "Compilation took:"
+--     let σ ← getDbgState
+--     logInfo m!"{←σ.pretty}"
+--     Sym.mkLambdaFVarsS args compiled
+--   Sym.shareCommonInc res
+
+section ExpressionAnalysis
+
+def _root_.Lean.Expr.pure? (e : Expr) : Option Expr :=
+  match_expr e with
+  | pure    _ _ _ x => .some x
+  | Option.some _ x => .some x
+  | _               => .none
+
+def _root_.Lean.Expr.bind? (e : Expr) : Option (Expr × Expr) :=
+  match_expr e with
+  | Bind.bind _ _ _ _ a f => .some (a, f)
+  | Option.bind   _ _ a f => .some (a, f)
+  | _                     => .none
+
+def _root_.Lean.Expr.bindInfo? (e : Expr) : Option (List Level × Array Expr) :=
+  match_expr e with
+  | Bind.bind _ _ α β a f => .some (e.getAppFn.constLevels!, #[α, β, a, f])
+  | Option.bind   α β a f => .some (e.getAppFn.constLevels!, #[α, β, a, f])
+  | _                     => .none
+
+end ExpressionAnalysis
+
+namespace Sets
+
+namespace Structural
+
+section pureBindMany
 
 /--
-info: Compiled:
-fun vec => eq0 (vec[0] + 1)
+`pure a₁ >>= fun _ : τ₁ ↦ pure a₂ >>= fun _ : τ₂ ↦ ...` ==>
+`[(a₁, τ₁, fun _ ↦ pure a₂ >>= fun _ ↦ ...), (a₂, τ₂, fun _ ↦ fun _ ↦ ...), ...]`
 -/
-#guard_msgs(info, whitespace := lax, drop warning) in
-#eval spoon <| do compileExampleJustSym ``ex₃ (←(map ∪ zeta ∪ getElem ∪ explode))
+partial def getBindPureLambdas (expr : Expr) : Option (List (Expr × Expr × Expr)) := do
+  let (_, #[α, _, a, f]) ← expr.bindInfo? | .none
+  let value ← a.pure?
+  let .lam (body := body) .. := f | .none
+  return (value, α, f) :: (←getBindPureLambdas body)
 
-def ex₄ (vec : Vector Nat 160) : Option Unit := do
-  let x ← vec.mapM (fun x ↦ return x + 1)
-  eq0 x[0]
+def substituteUnboundBvars (body : Expr) (values types : Array Expr) : Sym.SymM Expr := do
+  let wrappedBody := types.foldr (init := body) fun argType acc => .lam `x argType acc .default
+  return wrappedBody.beta values
+
+/-
+TODO this is currently extermely specialised and not correct in unhandled cases
+needs to also substitute into actions
+could do with perhaps calling the substitution function directly rather than beta reducing?
+-/
+def applyMany (body: Expr) (args: Array (Expr × Expr)) : Sym.SymM Expr := do
+  let mut args := args
+  for ((value, type), idx) in args.zipIdx do
+    let (values, types) := args.unzip
+    let value ← substituteUnboundBvars
+      value
+      (values.take idx)
+      (types.take idx)
+    let type ← substituteUnboundBvars
+      type
+      (values.take idx)
+      (types.take idx)
+    args := args.set! idx (value, type)
+  let (values, types) := args.unzip
+  substituteUnboundBvars body values types
 
 /--
-info: Compiled:
-fun vec => eq0 (vec[0] + 1)
--/
-#guard_msgs(info, whitespace := lax, drop warning) in
-#eval spoon <| do compileExampleJustSym ``ex₄ (←(mapM ∪ compilerSet_old ∪ getElem))
+A single-pass handling of `pure_bind` chains.
+In the spirit of `repeat rw [pure_bind]`.
 
-def ex₅ (vec : Vector Nat 3) : Option Unit := do
-  eq0 ((vec ++ vec)[0])
-  eq0 0
-  let res := vec.zipWith (bs := vec.map (·+1)) fun x y ↦ x + y
-  eq0 res[0]
-  eq0 res[1]
-  eq0 res[2]
+`pure a₁ >>= fun x ↦ pure a₂ >>= fun y ↦ f x y` ==> `f a₁ a₂`
+-/
+def pureBindMany : Sym.Simp.Simproc := fun expr ↦ do
+  match getBindPureLambdas expr with
+  | .none => return .rfl
+  | .some bindPurelambdas => 
+    let .some (_, _, f) := bindPurelambdas.getLast? | return .rfl
+    let .lam (body := body) .. := f | unreachable!
+    let expr' ← applyMany body (
+      bindPurelambdas.toArray.map fun (value, τ, _) => (value, τ)
+    )
+    trace[Clap.Compile.simp.proc.pureBindMany]
+      logRewrite expr expr' s!"Chained: {bindPurelambdas.length}"
+    return .step expr' (←mkSorry (←mkEq expr expr') false)
+
+end pureBindMany
+
+section flatten
+
+open Lean Meta in
+/--
+TODO: Make tail rec.
+
+A sequence of actions _in order_ as taken in a do block that is arbitrarily nested.
+Variables bound by the intermediate lambdas are reindexed to preserve data flow,
+i.e. interleaving the result with lambdas yields a semantically equivalent bind expression
+that is strictly right-linear.
+-/
+partial def sequenceActions (e : Expr) : Sym.Simp.SimpM (Array Expr) := do
+  go e [0]
+  where
+  go (e : Expr) (Γ : List ℕ) : Sym.Simp.SimpM (Array Expr) := do
+    match e.bind? with
+    | .some (action, func) =>
+      match action.bind? with
+      | .some (b, g) =>
+        let b ← go b Γ
+        let g ← go g Γ
+        let actions := b ++ g
+        /-
+          `let x ← do a₁; a₂; a₃; ...; aₙ` offsets subsequent lambdas `n - 1` times.
+          Note that `func` here is `λ x ↦ body`, so `x` is _bound_, i.e. not offset by
+          `liftLooseBVars`.
+        -/
+        let actions' ← go (func.liftLooseBVars 0 actions.size.pred) (actions.size :: Γ)
+        return actions ++ actions'
+      | _ =>
+        let func ← go func Γ
+        return #[action] ++ func
+    | _ =>
+      match e with
+      | .lam (body := body) .. =>
+        go body Γ
+      | _ =>
+        return #[e]
 
 /--
-info: Compiled:
-fun vec =>
-  (eq0 vec[0]).bind fun x =>
-    (eq0 0).bind fun x =>
-      (eq0 (vec[0] + (vec[0] + 1))).bind fun x =>
-        (eq0 (vec[1] + (vec[1] + 1))).bind fun x => eq0 (vec[2] + (vec[2] + 1))
+Optimises `bindActionsInferType`.
+TODO(untested)
+TODO(unused)
+TODO(perf) Should also grab universes...
 -/
-#guard_msgs(info, whitespace := lax, drop warning) in
-#eval spoon <| do
-  compileExampleJustSym
-    ``ex₅
-    (←(append ∪ explode ∪ getElem ∪ map ∪ zipWith ∪ zeta ∪ compilerSet_old))
-
-def ex₆ (vec : Vector Nat 160) : Option Unit := do
-  eq0 ((vec ++ vec)[0])
-  eq0 0
-  let res := (vec.drop 1).take 1
-  eq0 res[0]
+def _bindActions (a₁ a₁type a₂ a₂type: Expr) : Sym.Simp.SimpM (Expr × Expr) := do
+  let cont := Expr.lam `a a₁type a₂ default
+  let bind :=
+    mkApp4 (.const ``Option.bind [←Sym.getLevelInType a₁type, ←Sym.getLevelInType a₂type])
+           a₁type a₂type
+           a₁
+           cont
+  return (bind, a₂type)
 
 /--
-info: Compiled:
-fun vec => (eq0 vec[0]).bind fun x => (eq0 0).bind fun x => eq0 vec[1]
+Optimises `chainActionsInferType`.
+TODO(untested)
+TODO(unused)
+TODO(perf) Should also grab universes...
 -/
-#guard_msgs(info, whitespace := lax, drop warning) in
-#eval spoon <| do compileExampleJustSym ``ex₆ (←(append ∪ getElem ∪ drop ∪ take ∪ zeta ∪ compilerSet_old ∪ explode))
-
-def ex₇ (vec : Vector Nat 3) : Option Unit := do
-  eq0 ((vec ++ vec)[0])
-  eq0 0
-  let res := vec.sum
-  eq0 res
+def _chainActions (t : Expr) (actions : Array (Expr × Expr)) : Sym.Simp.SimpM Expr := do
+  let .some (action, _) := actions.back? | throwError m!"expected some action"
+  let actions := actions.pop
+  let (e', _) ← actions.foldrM (init := (action, t)) fun (a₁, ta₁) (a₂, ta₂) ↦
+    _bindActions a₁ ta₁ a₂ ta₂
+  let e' ← Sym.shareCommonInc e'
+  return e'
 
 /--
-info: Compiled:
-fun vec =>
-(eq0 vec[0]).bind fun x =>
-(eq0 0).bind fun x =>
-eq0 (vec[0] + (vec[1] + (vec[2] + 0)))
--/
-#guard_msgs(info, whitespace := lax, drop warning) in
-#eval spoon <| do compileExampleJustSym ``ex₇ (←(append ∪ getElem ∪ sum ∪ zeta ∪ compilerSet_old ∪ explode))
+A `bind a₁ λ x ↦ a₂ x` given `a₁` and `a₂`.
 
-def ex₈ (vec : Vector Nat 3) : Option Unit := do
-  let vec := vec.zipWith (·+·) #v[1, 5, 10]
-  eq0 42
-  let res ← vec.mapM (fun n ↦ return n + 1)
-  eq0 res[0]
-  eq0 res[1]
-  eq0 res[2]
+TODO(perf): Can cache types during traversal.
+-/
+def bindActionsInferType (action actionτ f fτ : Expr) : Sym.Simp.SimpM (Expr × Expr) := do
+  let cont := Expr.lam `a actionτ f .default
+  let bind :=
+    mkApp4 (.const ``Option.bind [←Sym.getLevelInType actionτ, ←Sym.getLevelInType fτ])
+           actionτ fτ
+           action
+           cont
+  return (bind, fτ)
 
 /--
-info: Compiled:
-fun vec =>
-(eq0 42).bind fun x =>
-(eq0 (vec[0] + 1 + 1)).bind fun x =>
-(eq0 (vec[1] + 5 + 1)).bind fun x =>
-eq0 (vec[2] + 10 + 1)
--/
-#guard_msgs(info, whitespace := lax, drop warning) in
-#eval spoon <| do compileExampleJustSym ``ex₈ (←(zipWith ∪ mapM ∪ getElem ∪ zeta ∪ compilerSet_old ∪ explode))
+A sequence of expressions from `actions` intercalated with single-argument lambdas.
 
-def ex₉ (vec : Vector Nat 160) : Option Unit := do
-  let res := (#v[0] ++ vec).extract 1 2
-  eq0 res[0]
+TODO(perf): Can cache types during traversal.
+-/
+def chainActionsInferType (actions : Array Expr) : Sym.Simp.SimpM Expr := do
+  let actions ← actions.mapM fun action ↦ do
+    let_expr Option τ := ←Sym.inferType action | throwError m!"expected option"
+    return (action, τ)
+  let .some action := actions.back? | throwError m!"expected some action"
+  let actions := actions.pop
+  let (e', _) ← actions.foldrM (init := action) fun (a₁, τ₁) (a₂, τ₂) ↦
+    bindActionsInferType a₁ τ₁ a₂ τ₂
+  let e' ← Sym.shareCommonInc e'
+  return e'
 
 /--
-info: Compiled:
-fun vec => eq0 vec[0]
+A flat sequence of actions from an expression that nests `bind`s arbitrarily.
+The result is thus a strict right-leaning linear tree of the form
+`a₀ >>= λ x₁ ↦ a₁ >>= λ x₂ ↦ ...`.
+
+E.g.
+`do a₀` 
+`   let x ← do a₁; a₂`
+`   a₃ x`
+==>
+`do a₀`
+`   a₁`
+`   let x ← a₂`
+`   a₃ x`
 -/
-#guard_msgs(info, whitespace := lax, drop warning) in
-#eval spoon <| do compileExampleJustSym ``ex₉ (←(extract ∪ append ∪ getElem ∪ zeta ∪ compilerSet_old ∪ explode))
+def flattenBindsAny : Sym.Simp.Simproc := fun e ↦ do
+  let .some (a, _) := e.bind? | return .rfl
+  let .some (_, _) := a.bind? | return .rfl
+  let e' ← sequenceActions e
+  let e' ← chainActionsInferType e'
+  return .step e' (←mkSorry (←mkEq e e') false)
 
-def ex₁₀ (vec : Vector Nat 160) : Option Unit := do
-  let res := (#v[0] ++ vec).set 0 42
-  eq0 res[0]
+end flatten
 
-/--
-info: Compiled:
-fun vec => eq0 42
--/
-#guard_msgs(info, whitespace := lax, drop warning) in
-#eval spoon <| do compileExampleJustSym ``ex₁₀ (←(set ∪ append ∪ getElem ∪ zeta ∪ compilerSet_old ∪ explode))
+def structural : MetaM Sym.Simp.Methods :=
+  mkMethods #[
+    (``pureBindMany, .Pre),
+    (``flattenBindsAny, .Pre)
+  ]
 
-def ex₁₁ (vec : Vector Nat 160) : Option Unit := do
-  let res := vec.mapIdx fun i x ↦ x + i
-  eq0 res[0]
+end Structural
 
-/--
-info: Compiled:
-fun vec => eq0 (vec[0] + 0)
--/
-#guard_msgs(info, whitespace := lax, drop warning) in
-#eval spoon <| do compileExampleJustSym ``ex₁₁ (←(mapIdx ∪ getElem ∪ zeta ∪ compilerSet_old ∪ explode))
+namespace General
 
-end ExampruSym
+def general : MetaM Sym.Simp.Methods := return {}
 
-end Clap.Compiler
+end General
+
+namespace Functional
+
+def functional : MetaM Sym.Simp.Methods := return {}
+
+end Functional
+
+end Sets
+
+open Sets in
+partial def consiliumMagnum (e : Expr) : Sym.Simp.SimpM Expr := do
+  ire e 0
+  where
+    simp (e : Expr) (symset : Sym.Simp.Methods) : Sym.Simp.SimpM Expr :=
+      Sym.simp e symset <&> (·.getResultExpr e)
+
+    consiliumStructurale (e : Expr) : Sym.Simp.SimpM Expr := do
+      simp e (←Structural.structural)
+    
+    consiliumFunctionale (e : Expr) : Sym.Simp.SimpM Expr := do
+      simp e (←Functional.functional)
+
+    consiliumGenerale (e : Expr) : Sym.Simp.SimpM Expr := do
+      simp e (←General.general)
+
+    ire (e : Expr) (numPasses : ℕ) : Sym.Simp.SimpM Expr := do
+      withTraceNode `Clap.Compile.consiliumMagnum.pass formatExprWith do
+
+      let e' ← withTraceNode `Clap.Compile.consiliumMagnum.pass.structurale formatExprWith do
+        consiliumStructurale e
+      
+      let e'' ← withTraceNode `Clap.Compile.consiliumMagnum.pass.functionale formatExprWith do
+        consiliumFunctionale e'
+
+      let e''' ← withTraceNode `Clap.Compile.consiliumMagnum.pass.generale formatExprWith do
+        consiliumGenerale e''
+      
+      if Sym.isSameExpr e e'''
+      then trace[Clap.Compile.consiliumMagnum] m!"Fixpoint reached after {numPasses} iterations."
+           trace[Clap.Compile.consiliumMagnum] m!"{logRewrite e e'''}"
+           return e'''
+      else ire e''' numPasses.succ    
+
+def compile (e : Expr) : Sym.Simp.SimpM Expr := do
+  let e ← Compiler.Simp.preprocessExpr e
+  let res ← lambdaTelescope e fun args e ↦ do
+    let (compiled, time) ← Dbg.timeS (consiliumMagnum e)
+    trace[Clap.Compile] m!"Compilation took: {time}s."
+    inDebugOnly (do getDbgState >>= fun σ ↦ do logInfo m!"{←σ.pretty}")
+    Sym.mkLambdaFVarsS args compiled
+  Sym.shareCommonInc res
+
+
+-- open Sym.Simp in
+-- /--
+-- TODO: Simp... STAHP?!
+-- -/
+-- private def actaStrategiaMagna : Simproc := fun e ↦ do
+--   let .some (us, #[α, β, a, f]) := e.matchBindsEInfo | return .rfl
+--   let simp (e : Expr) : Sym.Simp.SimpM Result := do Sym.simp e (←read).toMethods
+--   let ωₗ ← simp a
+--   let ωₗ := ωₗ.markAsDone.getResultExpr a
+--   trace[Clap.Compile.simp.proc.strategiaMagna]
+--     m!"Focus:\n{a}\nin:\n{e}\n==>ₗ\n{ωₗ}"
+--   let ωᵣ := f
+--   -- let ωᵣ ← simp f
+--   -- let ωᵣ := ωᵣ.getResultExpr f
+--   -- trace[Clap.Compile.simp.proc.strategiaMagna]
+--   --   m!"Focus:\n{f}\nin:\n{e}\n==>ᵣ\n{ωᵣ}"
+--   let e' := mkApp4 (.const ``Option.bind us) α β ωₗ ωᵣ
+--   return .step e' (←mkSorry (←mkEq e e') false)
+
+-- def strategiaMagna : MetaM Sym.Simp.Methods :=
+--   mkPreMethods #[
+--     ``actaStrategiaMagna
+--   ]
+
+end Dom
+
+end NewTraversal
+
+end Clap.Compiler.ExampruSym
