Clap/Compiler/Wheels.lean
@@ -1,88 +1,92 @@
 import Lean
--- import Lean.Util.PtrSet
--- import Lean.Declaration
 
-initialize Lean.registerTraceClass `Clap.Compiler
+open Lean
 
-/--
-`Clap.Compiler.preprocess` reports prime resolution and typeclass instantiation.
+initialize registerTraceClass `Clap.Compile
+
+
+initialize registerTraceClass `Clap.Compile.consiliumMagnum (inherited := true)
+
+initialize registerTraceClass `Clap.Compile.consiliumMagnum.pass (inherited := true)
+
+initialize registerTraceClass `Clap.Compile.consiliumMagnum.pass.structurale (inherited := true)
+
+initialize registerTraceClass `Clap.Compile.consiliumMagnum.pass.functionale (inherited := true)
+
+initialize registerTraceClass `Clap.Compile.consiliumMagnum.pass.generale (inherited := true)
+
+initialize registerTraceClass `Clap.Compile.simp (inherited := true)
+
+initialize registerTraceClass `Clap.Compile.simp.proc (inherited := true)
+
+initialize registerTraceClass `Clap.Compile.simp.proc.beta (inherited := true)
+initialize registerTraceClass `Clap.Compile.simp.proc.strategiaMagna (inherited := true)
+
+initialize registerTraceClass `Clap.Compile.simp.proc.kaboom (inherited := true)
+
+initialize registerTraceClass `Clap.Compile.simp.proc.getElem_mk (inherited := true)
+
+initialize registerTraceClass `Clap.Compile.simp.proc.mk_append_mk (inherited := true)
+
+initialize registerTraceClass `Clap.Compile.simp.proc.vector_mapM_mk_eq_append (inherited := true)
+
+initialize registerTraceClass `Clap.Compile.simp.proc.sequenceAsVecExpr (inherited := true)
+
+initialize registerTraceClass `Clap.Compile.simp.proc.zeta (inherited := true)
+
+initialize registerTraceClass `Clap.Compile.simp.proc.evalGround (inherited := true)
+
+initialize registerTraceClass `Clap.Compile.simp.proc.vector_getElem_mk (inherited := true)
+
+initialize registerTraceClass `Clap.Compile.simp.proc.vector_mk_zipWith_mk (inherited := true)
+
+initialize registerTraceClass `Clap.Compile.simp.proc.vector_mapM_mk (inherited := true)
+
+initialize registerTraceClass `Clap.Compile.simp.proc.vector_foldlM_mk (inherited := true)
+
+initialize registerTraceClass `Clap.Compile.simp.proc.vector_foldlM_stagger (inherited := true)
+
+initialize registerTraceClass `Clap.Compile.simp.proc.vector_mapIdx_mk (inherited := true)
+
+initialize registerTraceClass `Clap.Compile.simp.proc.vector_mk_append_mk (inherited := true)
+
+initialize registerTraceClass `Clap.Compile.simp.proc.vector_set_mk (inherited := true)
+
+initialize registerTraceClass `Clap.Compile.simp.proc.mapM_mk_single (inherited := true)
+
+initialize registerTraceClass `Clap.Compile.simp.proc.monad (inherited := true)
+
+initialize registerTraceClass `Clap.Compile.simp.proc.monad.bind_assoc (inherited := true)
+
+initialize registerTraceClass `Clap.Compile.simp.proc.monad.bind_eq_bind (inherited := true)
+
+initialize registerTraceClass `Clap.Compile.simp.proc.monad.bind_some (inherited := true)
+
+initialize registerTraceClass `Clap.Compile.simp.proc.monad.pure_apply (inherited := true)
+
+initialize registerTraceClass `Clap.Compile.simp.proc.monad.top_level (inherited := true)
+
+initialize registerTraceClass `Clap.Compile.simp.proc.preprocess (inherited := true)
+
+initialize registerTraceClass `Clap.Compile.simp.proc.flattenBinds (inherited := true)
+
+initialize registerTraceClass `Clap.Compile.simp.proc.pureBindMany (inherited := true)
+
+initialize registerTraceClass `Clap.Compile.simp.proc.seemsTotallySafeInDTT (inherited := true)
+
+initialize registerTraceClass `Clap.Compile.debug.simp (inherited := true)
+
+/-
+TODO: Having a `dbg` option and a `trace dbg` option is silly.
+That said, I want to treat a `traceClass` as a trace class only, I don't want
+to check it programatically whether it's on, to use as a debug flag as well.
 -/
-initialize Lean.registerTraceClass `Clap.Compiler.preprocess (inherited := true)
+initialize Lean.registerTraceClass `Clap.Compile.dbg (inherited := false)
 
-initialize Lean.registerTraceClass `Clap.Compiler.nameResolution (inherited := true)
-
-initialize Lean.registerTraceClass `Clap.Compiler.reduce (inherited := true)
-
-initialize Lean.registerTraceClass `Clap.Compiler.reduce.numIters (inherited := true)
-
-initialize Lean.registerTraceClass `Clap.Compiler.reduce.unfoldAny (inherited := true)
-
-initialize Lean.registerTraceClass `Clap.Compiler.reduce.dsimp (inherited := true)
-
-initialize Lean.registerTraceClass `Clap.Compiler.reduce.beta (inherited := true)
-
-initialize Lean.registerTraceClass `Clap.Compiler.reduce.zeta (inherited := true)
-
-initialize Lean.registerTraceClass `Clap.Compiler.reduce.linearise (inherited := true)
-
-initialize Lean.registerTraceClass `Clap.Compiler.reduce.foldProjs (inherited := true)
-
-initialize Lean.registerTraceClass `Clap.Compiler.reduce.letSome (inherited := true)
-
-initialize Lean.registerTraceClass `Clap.Compiler.serialise (inherited := true)
-
-initialize Lean.registerTraceClass `Clap.Compiler.curry (inherited := true)
-
-initialize Lean.registerTraceClass `Clap.Compile
-
-initialize Lean.registerTraceClass `Clap.Compile.traversal (inherited := true)
-
-initialize Lean.registerTraceClass `Clap.Compile.down (inherited := true)
-
-initialize Lean.registerTraceClass `Clap.Compile.up (inherited := true)
-
-initialize Lean.registerTraceClass `Clap.Compile.simp (inherited := true)
-
-initialize Lean.registerTraceClass `Clap.Compile.simp.fail (inherited := true)
-
-initialize Lean.registerTraceClass `Clap.Compile.simp.config (inherited := true)
-
-initialize Lean.registerTraceClass `Clap.Compile.simp.kaboom (inherited := true)
-
-initialize Lean.registerTraceClass `Clap.Compile.simp.warnDownNotGround (inherited := true)
-
-initialize Lean.registerTraceClass `Clap.Compile.simp.proc (inherited := true)
-
-initialize Lean.registerTraceClass `Clap.Compile.simp.proc.getElem_mk (inherited := true)
-
-initialize Lean.registerTraceClass `Clap.Compile.simp.proc.mk_append_mk (inherited := true)
-
-initialize Lean.registerTraceClass `Clap.Compile.simp.proc.vector_mapM_mk_eq_append (inherited := true)
-
-initialize Lean.registerTraceClass `Clap.Compile.simp.proc.sequenceAsVecExpr (inherited := true)
-
-initialize Lean.registerTraceClass `Clap.Compile.simp.proc.zeta (inherited := true)
-
-initialize Lean.registerTraceClass `Clap.Compile.simp.proc.evalGround (inherited := true)
-
-initialize Lean.registerTraceClass `Clap.Compile.simp.proc.vector_getElem_mk (inherited := true)
-
-initialize Lean.registerTraceClass `Clap.Compile.simp.proc.vector_mk_zipWith_mk (inherited := true)
-
-initialize Lean.registerTraceClass `Clap.Compile.simp.proc.vector_mapM_mk (inherited := true)
-
-initialize Lean.registerTraceClass `Clap.Compile.simp.proc.vector_mapIdx_mk (inherited := true)
-
-initialize Lean.registerTraceClass `Clap.Compile.simp.proc.vector_mk_append_mk (inherited := true)
-
-initialize Lean.registerTraceClass `Clap.Compile.simp.proc.vector_set_mk (inherited := true)
-
-initialize Lean.registerTraceClass `Clap.Compile.simp.proc.preprocess (inherited := true)
-
-initialize Lean.registerTraceClass `Clap.Compile.simp.proc.seemsTotallySafeInDTT (inherited := true)
-
-initialize Lean.registerTraceClass `Clap.Compile.debug.simp (inherited := true)
-
+register_option Clap.Compile.dbg : Bool := {
+  defValue := false
+  descr := "global debugging state"
+}
 
 open Lean Elab.Term in
 def formatExprWith {m : Type _ → Type _} [Monad m]
@@ -110,7 +114,6 @@ def Lean.Meta.forallTelescopeOne!.{u}
 open Lean Meta Sym Elab in
 def Lean.Meta.Sym.Simp.liftTermElabM {α} (m : TermElabM α) : Sym.Simp.SimpM α := liftM m.run'
 
-
 section
 
 open Lean.Meta
@@ -130,65 +133,39 @@ def Clap.SymSets.General.ground : MetaM Sym.Simp.Methods := do
 def Lean.Meta.Sym.simpWithGround (e : Expr) : SymM Sym.Simp.Result :=
   Clap.SymSets.General.ground >>= (Sym.simp e ·)
 
+def Lean.Meta.Sym.simpWithGround! (e : Expr) : SymM Expr := do
+  let res ← Clap.SymSets.General.ground >>= (Sym.simp e ·)
+  return res.getResultExpr e
+
 end
 
-def Clap.Dbg.timeInSecondsOfMs (begin «end» : Nat) : Float :=
+namespace Clap.Dbg
+
+def timeInSecondsOfMs (begin «end» : Nat) : Float :=
   (Float.ofNat «end» - Float.ofNat begin) / Float.ofNat 1000
 
-def Clap.Dbg.timeSince (begin : Nat) (msg := ""): Lean.Meta.Sym.Simp.SimpM Unit := do
+def timeSince (begin : Nat) (msg := ""): Lean.Meta.Sym.Simp.SimpM Unit := do
   Lean.logWarning m!"{msg}\n{(Float.ofNat (←IO.monoMsNow) - Float.ofNat begin) / Float.ofNat 1000}s"
 
-register_simp_attr dbgSimp
+open Lean Meta Sym in
+def timeS {α} {m : Type _ → Type _} [Monad m] [MonadLiftT BaseIO m] (k : m α) : m (α × Float) := do
+  let s ← IO.monoNanosNow
+  let a ← k
+  let e ← IO.monoNanosNow
+  return (a, (e - s).toFloat / 1_000_000_000)
 
-register_simp_attr compilerSimp
+def inDebugOnly (m : Lean.Meta.Sym.Simp.SimpM Unit) : Lean.Meta.Sym.Simp.SimpM Unit := do
+  if (←getBoolOption ``Clap.Compile.dbg) then
+    m
 
--- /-
--- Based on `Expr.getUsedConstants`.
--- -/
+end Clap.Dbg
 
--- namespace Lean
--- namespace Expr
--- namespace FoldConstsImpl
+def Lean.Name.lastComponent! (name : Name) : Name := name.componentsRev.head!
 
--- unsafe structure State' where
---  visited       : PtrSet Expr := mkPtrSet
---  visitedConsts : NameHashSet := {}
-
--- unsafe def fold' {α : Type} (f : Name → α → α) (e : Expr) (acc : α) : StateT State MetaM α :=
---   let rec visit (e : Expr) (acc : α) : StateT State MetaM α := do
---     if (←Meta.inferType e).isProp then
---       logInfo m!"Rejected: {e} with T: {←Meta.inferType e}"
---       return acc
---     if (← get).visited.contains e then
---       return acc
---     modify fun s => { s with visited := s.visited.insert e }
---     match e with
---     | .forallE _ d b _   => visit b (← visit d acc)
---     | .lam _ d b _       => visit b (← visit d acc)
---     | .mdata _ b         => visit b acc
---     | .letE _ t v b _    => visit b (← visit v (← visit t acc))
---     | .app f a           => visit a (← visit f acc)
---     | .proj _ _ b        => visit b acc
---     | .const c _         =>
---       if (← get).visitedConsts.contains c then
---         return acc
---       else
---         modify fun s => { s with visitedConsts := s.visitedConsts.insert c };
---         return f c acc
---     | _ => return acc
---   visit e acc
-
--- @[inline] unsafe def foldUnsafe' {α : Type} (e : Expr) (init : α) (f : Name → α → α) : MetaM α :=
---   (fold' f e init).run' {}
-
--- end FoldConstsImpl
-
--- /-- Apply `f` to every constant occurring in `e` once. -/
--- @[implemented_by FoldConstsImpl.foldUnsafe']
--- opaque foldConsts' {α : Type} (e : Expr) (init : α) (f : Name → α → α) : MetaM α := return init
-
--- def getUsedConstants' (e : Expr) : MetaM (Array Name) :=
---   e.foldConsts' #[] fun c cs => cs.push c
-
--- end Expr
--- end Lean
+theorem List.drop_toArray {α} {l : List α} {i} :
+  l.toArray.drop i = (l.drop i).toArray := by
+  simp only [
+    Array.drop_eq_extract, List.size_toArray, List.extract_toArray,
+    List.extract_eq_take_drop, Array.mk.injEq
+  ]
+  rw [←List.extract_eq_take_drop, List.drop_eq_extract]
