Clap/Test/Compiler/Traverse/Down.lean
@@ -1,0 +1,339 @@
+import Clap.Test.Compiler.Traverse.Prelude
+
+namespace ExampruSym
+
+namespace NewTraversal
+
+open Clap.Compiler
+
+def testInnerReturn : Option ℕ := do
+  let x ← F 1
+  let y ← F (←(fun (x: ℕ) => do
+    return x) 3)
+  let z ← F 3
+  pure z
+
+#eval Lean.ToExpr.toExpr testInnerReturn
+
+-- Environment.find? ``testInnerReturn
+
+set_option trace.Clap.Compile true in
+set_option Clap.traversalDbg true in
+set_option trace.Clap.Compile.dbg true in
+#eval runTestByName ``testInnerReturn (isUsingTopLevelStrategy := true) (eval := false)
+
+#exit
+
+def testRightBind : Option ℕ := do
+  let x ← F 1
+  let y ← F (x + 10)
+  return y
+set_option trace.Clap.Compile true in
+set_option Clap.traversalDbg true in
+set_option trace.Clap.Compile.dbg true in
+#eval runTestByName ``testRightBind (isUsingTopLevelStrategy := true)
+
+def testLeftBind : Option ℕ := do
+  let y ← F ((←do
+    let x ← F 1;
+    return x) + 10
+  )
+  return y
+set_option trace.Clap.Compile true in
+set_option Clap.traversalDbg true in
+set_option trace.Clap.Compile.dbg true in
+#eval runTestByName ``testLeftBind
+
+
+-- def testTreeBind : Option ℕ := do
+--   let y ← F ((←do
+--     let x ← F 1;
+--     let y ← F (x + 10)
+--     return y) + 100
+--   )
+--   let z ← F ((←do
+--     let x ← F 1000;
+--     let y ← F (x + 10000)
+--     return y) + 100000
+--   )
+--   return y + z
+
+def testTreeBindNested : Option ℕ := do
+  let a ← F 1
+  let B ← F 2
+  let b ← (
+    do let x ← F (a + B)
+       let y ← F (x + 10)
+       let z ← F (x + 42)
+       return y + y + B + z
+  )
+  let w ← F (b + 100)
+  let y ← F (b + 200)
+  let c ← (
+    do let x ← F 1000;
+       let y ← F (x + 10000)
+       let z ← (do
+         let a ← F 3
+         let b ← F (a + w)
+         let c ← F (a + b)
+         let d ← F 4
+         return c + d)
+       return y + a + w + z + B + w
+  )
+  let z ← F (c + 100000)
+  return y + z + a + b
+
+def flattenedTreeBindNested : Option ℕ := do
+  let a ← F 1
+  let B ← F 2
+  let x ← F (a + B)
+  let y ← F (x + 10)
+  let z ← F (x + 42)
+  let b ← pure (y + y + B + z)
+  let w ← F (b + 100)
+  let y ← F (b + 200)
+  let x ← F 1000;
+  let y' ← F (x + 10000)
+  let a' ← F 3
+  let b' ← F (a' + w)
+  let c' ← F (a' + b')
+  let d' ← F 4
+  let y'' ← pure (c' + d')
+  let c ← pure (y' + a + w + y'' + B + w)
+  let z ← F (c + 100000)
+  return y + z + a + b
+
+def testTreeBind : Option ℕ := do
+  let b ← (
+    do let x ← F 1
+       let y ← F (x + 10)
+       return y
+  )
+  let y ← F (b + 100)
+  let c ← (
+    do let x ← F 1000;
+       let y ← F (x + 10000)
+       return y
+  )
+  let z ← F (c + 100000)
+  return y + z -- `#2 + #0`
+
+def flattenedTreeBind : Option ℕ := do
+  let x ← F 1
+  let y ← F (x + 10)
+  let y ← pure y
+  let y ← F (y + 100)
+  let x ← F 1000
+  let y' ← F (x + 10000)
+  let y' ← pure y'
+  let z ← F (y' + 100000)
+  pure (y + z) -- `#4 + #0`
+
+example : flattenedTreeBind = testTreeBind := by
+  unfold flattenedTreeBind testTreeBind
+  simp [bind_assoc, Option.bind_assoc]
+
+open Lean Meta in
+/--
+TODO: Make tail rec.
+-/
+partial def planusEst (e : Expr) : Sym.Simp.SimpM (Array Expr) := do
+  let res ← go e [0]
+  logInfo m!"res: {res}"
+  return res
+  where
+  go (e : Expr) (Γ : List ℕ) : Sym.Simp.SimpM (Array Expr) := do
+    trace[Clap.Compile.dbg] m!"e[{Γ}]:\n{e}"
+    match e.matchBindsE with
+    | .some (action, func) =>
+      match action.matchBindsE with
+      | .some (b, g) =>
+        let b ← go b Γ
+        let g ← go g Γ
+        let actions := b ++ g
+        -- `let x ← do a₁; a₂; a₃; ...; aₙ` offsets subsequent lambdas `n - 1` times
+        logInfo m!"func: {func}"
+        logInfo m!"↑[{actions.size.pred}]"
+        let actions' ← go (func.liftLooseBVars 0 actions.size.pred) (actions.size :: Γ)
+        return actions ++ actions'
+      | _ =>
+        let func ← go func Γ
+        return #[action] ++ func
+    | _ =>
+      match e with
+      | .lam (body := body) .. =>
+        go body Γ
+      | _ =>
+        return #[e]
+
+-- open Lean in
+-- partial def planusEst' (e : Expr) (level : ℕ) (count : ℕ) (lams : ℕ) (lr : LR) : MetaM ℕ := do
+--   let newLevel := newLevel (level := level)
+--   -- logInfo m!"e[l={level}][c={count}][λ={lams}]:\n{e}"
+--   if let .some (a, f) := e.matchBindsE
+--   then
+--     let level' := newLevel a
+--     if level' != level then logInfo m!"push: {a}"
+--     let left ← planusEst' a level' count lams Left
+--     if level' != level then logInfo m!"pop"
+--     let right ← planusEst' f level count lams Right
+--     if level' != level then logInfo m!"left: {left} | right: {right}\ne: {e}\nrepl: {e.liftLooseBVars 0 left}"
+--     return left + right
+--   else
+--     match e with
+--     | .lam (body := body) .. =>
+--       -- logInfo m!"lam[l={level}][c={count}][λ={lams}]: {e}"
+--       planusEst' body level count lams.succ lr
+--     | _ =>
+--       logInfo m!"any[l={level}][c={count}][λ={lams}]:\n{e}\n==>\n{e.liftLooseBVars 1 count}"
+--       return count.succ
+    
+
+  --   if let .some (b, g) := a.matchBindsE
+  --   then
+  --     let level := level.succ
+  --     let count := 0
+  --     let left ← planusEst a level count Left
+  --     -- let count := left
+  --     let right ← planusEst f level count Right
+  --     logInfo m!"blocksize|L: {left} R: {right}"
+  --     return left + right
+  --   else
+  --     let level := level
+  --     let count := count
+  --     let left ← planusEst a level count Left
+  --     -- let count := left
+  --     let right ← planusEst f level count Right
+  --     logInfo m!"blocksize|L: {left} R: {right}"
+  --     return right.succ
+  -- else
+  -- match e with
+  -- | .lam (body := body) .. =>
+  --   logInfo m!"lam[l={level}][c={count}]: {e}"
+  --   planusEst body level count lr
+  -- | _ => logInfo m!"any[l={level}][c={count}]: {e}"; return count.succ
+
+set_option trace.Clap.Compile.dbg true in
+open Lean in
+run_meta do
+  let rec go (e : Expr) : MetaM Unit :=
+    match e with
+    | .bvar .. => logInfo m!"{e}"
+    | e => discard (e.traverseChildren (fun e ↦ go e >>= fun _ ↦ return e))
+  
+  -- let tree := (←getEnv).find? ``testTreeBind |>.get!.value!
+  -- let flattree := (←getEnv).find? ``flattenedTreeBind |>.get!.value!
+  let testTreeBindNested := (←getEnv).find? ``testTreeBindNested |>.get!.value!
+  let flatNested := (←getEnv).find? ``flattenedTreeBindNested |>.get!.value!
+
+  -- logInfo m!"{repr tree}"
+  -- logInfo m!"{repr flattree}"
+
+  -- let res ← (planusEst tree).run'.run
+  -- logInfo m!"res: {res}"
+
+  let res ← (planusEst testTreeBindNested).run'.run
+  logInfo m!"resNested: {res}"
+                        -- [1, 0, 0, 0, 0, 2, 0, 1, 0, 0, 8, 3, 0, 4, 0, 10, 6]
+
+  logInfo m!"not flat:"
+  go testTreeBindNested -- [1, 0, 0, 0, 0, 2, 0, 1, 0, 0, 6, 3, 0, 2, 0, 6, 4]
+  logInfo m!"flat:"
+  go flatNested
+  -- [#1, #0, #0, #1 ,#1 ,#1 ,#3 ,#0 ,#0 ,#1 ,#0 ,#0 ,#4 ,#1 ,#0 ,#1 ,#0 ,#5 ,#14 ,#8 ,#0 ,#0 ,#9 ,#0 ,#16 ,#11] 
+
+  -- logInfo m!"not flat:"
+  -- go tree
+  -- logInfo m!"flat:"
+  -- go flattree
+
+
+
+  
+
+example :
+  testTreeBind =
+  (((F 1).bind fun x => (F (x.add 10)).bind fun y => some y).bind fun __do_lift =>
+    (F (__do_lift.add 100)).bind fun y =>
+      ((F 1000).bind fun x => (F (x.add 10000)).bind fun y => some y).bind fun __do_lift =>
+        (F (__do_lift.add 100000)).bind fun z => some (y.add z))
+:=
+  rfl
+  -- by
+  -- unfold testTreeBind
+  -- unfold_projs
+
+example :
+  testTreeBind = flattenedTreeBind
+:= by
+  simp only [
+    testTreeBind,
+    flattenedTreeBind
+  ]
+  simp only [
+    bind_assoc
+  ]
+
+#print testTreeBind
+set_option trace.Clap.Compile true in
+set_option Clap.traversalDbg true in
+set_option trace.Clap.Compile.dbg true in
+#eval runTestByName ``testTreeBind
+
+set_option trace.Clap.Compile true in
+set_option Clap.traversalDbg true in
+set_option trace.Clap.Compile.dbg true in
+#eval runTestByName ``testTreeBindNested
+
+def exex' : Option ℕ := do
+  let z ← F 2
+  let x ← H 4
+  let y ← (do let x ← G (x + z); let y ← G x; H (x + z))
+  H y
+#check @Option.bind_assoc
+set_option trace.Clap.Compile true in
+set_option Clap.traversalDbg true in
+set_option trace.Clap.Compile.dbg true in
+#eval runTestByName ``exex'
+
+def exex'' : Option ℕ := do
+  let z ← F 2
+  let x ← #v[1, 2, 3, 4].mapM (fun _ ↦ pure 4)
+  let y ← (do let x ← G x[0]; let y ← G x; H (x + z))
+  H y
+
+#check @Option.bind_assoc
+set_option trace.Clap.Compile true in
+set_option Clap.traversalDbg true in
+set_option trace.Clap.Compile.dbg true in
+#eval runTestByName ``exex''
+
+opaque A : Nat → Option Nat
+opaque B : Nat → Option Nat
+opaque C : Nat → Option Nat
+opaque D : Nat → Option Nat
+opaque E : Nat → Option Nat
+
+def eboom (vec : Vector Nat 4) : Option Unit := do
+  let x ←
+    (do
+      let _ ← A 0
+      let x ←
+        (do let y ← do
+            let _ ← B 1
+            let res ←
+              (do let w ← C 2
+                  D 5)
+            E res)
+      F x
+    )
+  discard (G x)
+
+-- set_option trace.Clap.Compile true in
+-- set_option Clap.traversalDbg true in
+-- set_option trace.Clap.Compile.dbg true in
+-- #eval runTestByName ``eboom
+
+end NewTraversal
+
+namespace ExampruSym
