Clap/Test/Compiler/Traverse/Foldlm.lean
@@ -1,0 +1,41 @@
+import Clap.Test.Compiler.Traverse.Prelude
+
+namespace ExampruSym
+
+namespace NewTraversal
+
+open Clap.Compiler
+
+opaque share : ℕ → Option ℕ
+
+-- abbrev sigma (x : ℕ) : Option (ℕ) := do
+--   let x2 ← share (x * x)
+--   let x4 ← share (x2 * x2)
+--   some (x4 * x)
+
+abbrev sigma_unshared (x : ℕ) : Option (ℕ) := do
+  let x2 ← some (x + x)
+  let x4 ← some (x2 + x2)
+  some (x4 + x)
+
+def testFoldlM : Option ℕ := do
+  let xs ← (List.range 64).foldlM (fun state r ↦ do
+    let s0 ← sigma_unshared state[0]
+    state.set 0 s0
+    ) #v[0, 1, 2]
+  let x ← xs[0]
+  return x
+
+-- set_option trace.Clap.Compile.simp.consiliumMagnum true in
+-- set_option trace.Clap.Compile.simp.proc.vector_foldlM_stagger true in
+-- set_option Clap.traversalDbg true in
+-- set_option trace.Clap.Compile.dbg true in
+-- -- set_option pp.exprSizes true in
+-- set_option trace.Clap.Compile.simp.proc.beta true in
+set_option maxRecDepth 100000 in
+-- set_option maxHeartbeats 800000 in
+#eval runTestByName ``testFoldlM false true
+
+end NewTraversal
+
+end ExampruSym
