Clap/Test/Compiler/Traverse/Misc.lean
@@ -1,0 +1,525 @@
+import Clap.Test.Compiler.Traverse.Prelude
+
+namespace ExampruSym
+
+open SymSets Monad General Vector
+
+def exex : Option Unit :=
+  Option.bind (eq0 4) fun _ : Unit ↦
+    Option.bind
+      ((Option.bind
+         (Option.bind
+           (Option.bind
+             (F 2) fun x ↦
+            Option.bind (F 3) fun y ↦ G (x + y))
+           fun x ↦ H x))
+         fun x ↦ F x) fun x ↦
+      F x
+
+#print exex
+
+namespace NewTraversal
+
+def testInnerReturn : Option Unit := do
+  let x ← F 1
+  let y ← F (←(fun (x: ℕ) => do
+    return x) 3)
+  let z ← F 3
+  pure ()
+
+set_option trace.Clap.Compile true in
+set_option Clap.traversalDbg true in
+set_option trace.Clap.Compile.dbg true in
+#eval spoon <| do
+  let e ← compileExample ``testInnerReturn (←(mapM_singlePass_pre))
+  -- Pretty print (i.e. go back to `Bind.bind`)
+  return (←Sym.simp e (←compilerBindEqBind)).getResultExpr e
+
+
+def exex' : Option Unit := do
+  let z ← F 2
+  let x ← H 4
+  let y ← (do let x ← G (x + z); let y ← G x; H (x + z))
+  H y
+
+def exex'' : Option Unit := do
+  let z ← F 2
+  let x ← #v[1, 2].mapM (fun _ ↦ pure 4)
+  let y ← (do let x ← G x[1]; let y ← G x; H (x + z))
+  H y
+
+#check @Option.bind_assoc
+
+set_option trace.Clap.Compile true in
+set_option Clap.traversalDbg true in
+set_option trace.Clap.Compile.dbg true in
+#eval spoon <| do
+  let e ← compileExample ``exex'' (←(mapM_singlePass_pre))
+  -- Pretty print (i.e. go back to `Bind.bind`)
+  return (←Sym.simp e (←compilerBindEqBind)).getResultExpr e
+
+end NewTraversal
+
+#exit
+
+-- set_option maxRecDepth 500000
+-- set_option trace.Clap.Compile true
+
+def ex₀ : Option Unit := do
+  eq0 0
+  eq0 1
+  let _res ← ([0, 1].foldlM (init := ()) fun _ _ ↦ eq0 2)
+  eq0 3
+  return ()
+
+/--
+info: Compiled:
+do
+  eq0 0
+  eq0 1
+  do
+    eq0 2
+    let init ← eq0 2
+    some init
+  eq0 3
+  some PUnit.unit
+-/
+#guard_msgs(info, whitespace := lax, drop warning) in
+#eval do spoon (compileExampleJustSym ``ex₀ (←(foldlM ∪ monads)))
+
+set_option trace.Clap.Compile true in
+#eval do spoon (compileExample ``ex₀ (←(foldlM)))
+
+-- mkPostMethodsSinglePass
+
+def ex₁ (_vec : Vector Nat 3) : Option Unit := do
+  eq0 #v[4, 5][0]
+
+/--
+info: Compiled:
+fun _vec => eq0 4
+-/
+#guard_msgs(info, whitespace := lax, drop warning) in
+#eval spoon <| do compileExampleJustSym ``ex₁ (←getElem)
+
+set_option trace.Clap.Compile true in
+#eval spoon <| do compileExample ``ex₁ (←getElem)
+
+/--
+info: Compiled:
+fun _vec => eq0 4
+-/
+#guard_msgs(info, whitespace := lax, drop warning) in
+#eval spoon <| do compileExample ``ex₁ (←getElem)
+
+def ex₂ (vec : Vector Nat 160) : Option Unit := do
+  let x := (vec ++ vec)[0] -- `GetElem (Vector _ (3 + 3))`
+  eq0 x
+-- /--
+-- info: Compiled:
+-- fun vec => eq0 vec[0]
+-- -/
+-- #guard_msgs(info, whitespace := lax, drop warning) in
+#eval spoon <| do compileExampleJustSym ``ex₂ (←(getElem ∪ append ∪ zeta ∪ explode))
+
+def ex₃ (vec : Vector Nat 200) : Option Unit := do
+  let x := vec.map (·+1)
+  eq0 x[0]
+
+/--
+info: Compiled:
+fun vec => eq0 (vec[0] + 1)
+-/
+#guard_msgs(info, whitespace := lax, drop warning) in
+#eval spoon <| do compileExampleJustSym ``ex₃ (←(map ∪ zeta ∪ getElem ∪ explode))
+
+def ex₄ (vec : Vector Nat 5) : Option Unit :=
+  vec.mapM (fun x ↦ Option.some <| x + 1) |>.bind fun x ↦ eq0 x[0]
+
+-- -- /--
+-- -- info: Compiled:
+-- -- fun vec => eq0 (vec[0] + 1)
+-- -- -/
+-- -- #guard_msgs(info, whitespace := lax, drop warning) in
+-- set_option pp.exprSizes true in
+-- -- set_option trace.Clap.Compile true in
+-- set_option trace.Clap.Compile.simp.proc.vector_mapM_mk true in
+-- set_option trace.profiler true in
+-- set_option profiler true in
+-- set_option trace.Clap.Compile true in
+set_option trace.Clap.Compile true in
+#eval spoon <| do
+  compileExampleJustSym ``ex₄
+    (←(mapM_alt ∪ monads ∪ getElem ∪ explode ∪ bindMyAssoc_set ∪ append))
+
+def profileThis := spoon <| do compileExampleJustSym ``ex₄ (←(mapM ∪ monads ∪ getElem))
+
+def reportAttempt : Sym.Simp.Simproc := fun e ↦ do
+  discard bump
+  return .rfl
+
+def reportSet : MetaM Sym.Simp.Methods :=
+  mkPreMethods #[
+    ``reportAttempt
+  ]
+
+
+def ex₅ (vec : Vector Nat 10) : Option Unit := do
+  eq0 ((vec ++ vec)[0])
+  eq0 0
+  let res := vec.zipWith (bs := vec.map (·+1)) fun x y ↦ x + y
+  eq0 res[0]
+  eq0 res[1]
+  eq0 res[2]
+
+set_option trace.Clap.Compile true in
+set_option maxRecDepth 100000 in
+-- /--
+-- info: Compiled:
+-- fun vec =>
+--   (eq0 vec[0]).bind fun x =>
+--     (eq0 0).bind fun x =>
+--       (eq0 (vec[0] + (vec[0] + 1))).bind fun x =>
+--         (eq0 (vec[1] + (vec[1] + 1))).bind fun x => eq0 (vec[2] + (vec[2] + 1))
+-- -/
+-- #guard_msgs(info, whitespace := lax, drop warning) in
+#eval spoon <| do
+  let res ← compileExampleJustSym
+    ``ex₅
+    (←(reportSet ∪ append ∪ explode ∪ getElem ∪ map ∪ zipWith ∪ zeta ∪ monads))
+  logInfo m!"this many times: {←getCounter}"
+  return res
+
+
+def ex₆ (vec : Vector Nat 160) : Option Unit := do
+  eq0 ((vec ++ vec)[0])
+  eq0 0
+  let res := (vec.drop 1).take 1
+  eq0 res[0]
+
+/--
+info: Compiled:
+fun vec => (eq0 vec[0]).bind fun x => (eq0 0).bind fun x => eq0 vec[1]
+-/
+#guard_msgs(info, whitespace := lax, drop warning) in
+#eval spoon <| do compileExampleJustSym ``ex₆ (←(append ∪ getElem ∪ drop ∪ take ∪ zeta ∪ monads ∪ explode))
+
+-- `f (λ f (λ g #1 #0))`
+-- `[0:#1, 1:#0, 2:g, 3: 2 1, 4: 3 1, 5: λ 4, 6: f, 7: λ 6 5, 8: 6 7]`
+-- `f ==> f'`
+-- `[0:#1, 1:#0, 2:g, 3: 2 1, 4: 3 1, 5: λ 4, 6: f, 7: λ 6 5, 8: 6 7, 9: f']`
+--
+
+def ex₇ (vec : Vector Nat 3) : Option Unit := do
+  eq0 ((vec ++ vec)[0])
+  eq0 0
+  let res := vec.sum
+  eq0 res
+
+-- def compile (e : Expr) : (Expr, Name) :=
+--   match_expr e with
+--   | Option.bind _ _ a f =>
+--     match_expr a with
+--     | Option.some _ x =>
+--       let e' : Expr := f.beta #[x]
+--       (e', ``LawfulMonad.bind_some)
+--     | _ => e
+--   | _ => e
+
+-- set_option trace.Clap.Compile true
+-- -- /--
+-- -- info: Compiled:
+-- -- fun vec =>
+-- -- (eq0 vec[0]).bind fun x =>
+-- -- (eq0 0).bind fun x =>
+-- -- eq0 (vec[0] + (vec[1] + (vec[2] + 0)))
+-- -- -/
+-- #guard_msgs(info, whitespace := lax, drop warning) in
+#eval spoon <| do compileExampleJustSym ``ex₇ (←(append ∪ getElem ∪ sum ∪ zeta ∪ monads ∪ explode))
+
+def ex₈ (n : ℕ) (vec : Vector Nat n) : Option Unit := do
+  let x ← (do let _ ← eq0 2; let X ← vec.mapM (fun x ↦ (eq0 (x + 42) : Option _)); return 4)
+  eq0 x
+
+def ex₈_fixed (vec : Vector Nat 2) : Option Unit := do
+  let x ← (do let _ ← eq0 2; let X ← vec.mapM (fun x ↦ (eq0 (x + 42) : Option _)); return 4)
+  eq0 x
+
+  -- let res ← vec.mapM (fun n ↦ return n + 1)
+  -- eq0 res[0]
+  -- let y ← (do eq0 4; let y ← pure 4; let z ← #v[1, 2].mapM (return·+42); eq0 z[0]; return y)
+  -- let z := (List.range y)[0]'sorry
+  -- eq0 res[1]
+  -- eq0 res[2]
+
+-- def ex₈' (vec : Vector Nat 100) : Option Unit := do
+--   let x ← (do let _ ← eq0 2; let _ ← vec.foldlM (fun acc x ↦ (eq0 (x + 42) : Option _)) (()); return 4)
+--   eq0 x
+--   -- let res ← vec.mapM (fun n ↦ return n + 1)
+--   -- eq0 res[0]
+--   -- let y ← (do eq0 4; let y ← pure 4; let z ← #v[1, 2].mapM (return·+42); eq0 z[0]; return y)
+--   -- let z := (List.range y)[0]'sorry
+--   -- eq0 res[1]
+--   -- eq0 res[2]
+#check bind_assoc
+set_option pp.exprSizes true in
+set_option trace.Clap.Compile true in
+set_option maxRecDepth 4000 in
+set_option maxHeartbeats 0 in
+-- set_option pp.exprSizes true in
+-- /--
+-- info: Compiled:
+-- fun vec =>
+--   (eq0 42).bind fun x =>
+--     (eq0 (vec[0] + 1 + 1)).bind fun x =>
+--       ((eq0 4).bind fun x => (eq0 (1 + 42)).bind fun x => some 4).bind fun y =>
+--         (eq0 (vec[1] + 5 + 1)).bind fun x => eq0 (vec[2] + 10 + 1)
+-- -/
+-- #guard_msgs(info, whitespace := lax, drop warning) in
+
+#eval spoon <| do
+  let (e, time) ← Dbg.timeS <| compileExampleJustSym ``ex₈_fixed
+    (←(reportSet ∪ mapM_alt ∪ zeta ∪ monads ∪ explode
+    -- ∪ compilerAssoc
+    ∪ bindMyAssoc_set
+    -- mapM_alt
+    ))
+  logInfo m!"Compilation took: {time}s"
+  -- logInfo m!"this many times: {←getCounter}"
+  -- Pretty print (i.e. go back to `Bind.bind`)
+  return (←Sym.simp e (←compilerBindEqBind)).getResultExpr e
+
+-- def xx : MetaM Sym.Simp.Methods :=
+
+-- set_option trace.Clap.Compile.dbg true in
+-- set_option Clap.traversalDbg true in
+-- set_option trace.Clap.Compile true in
+-- #eval spoon <| do
+--   resetDbgState
+--   let e ← compileExample (args := #[toExpr 160]) ``ex₈
+--     (←(mapM_singlePass ∪ zeta ∪ monads ∪ explode
+--     -- ∪ compilerAssoc
+--     -- ∪ bindMyAssoc_set
+--     -- mapM_alt
+--     ))
+--   let σ ← getDbgState
+--   logInfo m!"σ: {repr σ}"
+
+--   return e
+--   -- Pretty print (i.e. go back to `Bind.bind`)
+--   -- return (←Sym.simp e (←compilerBindEqBind)).getResultExpr e
+
+set_option maxRecDepth 1024 in
+set_option trace.Clap.Compile.dbg true in
+set_option Clap.traversalDbg true in
+set_option trace.Clap.Compile false in
+#eval do
+  let (e, time) ← Dbg.timeS <| compileExample (args := #[toExpr 5]) ``ex₈
+    (←(SymSets.Vector.wrapped ∪
+      mapM_singlePass_pre ∪
+      explode -- ∪ zeta ∪ monads ∪ explode
+    -- ∪ compilerAssoc
+    ∪ bindMyAssoc_set
+    -- mapM_alt
+    )) |>.run' {} |>.run
+  logInfo m!"time: {time}"
+  let e' := Sym.simp e (←compilerBindEqBind)
+  let e' ← e'.run
+
+  logInfo m!"e: {e'.getResultExpr e}"
+  logInfo m!"{←(getAndResetDbgState <&> repr)}"
+  -- return e
+
+-- set_option trace.Clap.Compile true
+-- set_option trace.Clap.Compile.up true
+set_option Clap.traversalDbg true
+set_option trace.Clap.Compile.dbg false
+def bench : MetaM Unit := do
+  let simpset := (←(SymSets.Vector.wrapped ∪ mapM_singlePass_pre ∪ explode ∪ compilerAssoc))
+  -- let simpset := (←(mapM_singlePass ∪ zeta ∪ explode))
+  let inputSizes := (Array.range 2).map (10 * 2^·)
+  let timings ← inputSizes.mapM fun inputSize ↦ do
+    let res ← Dbg.timeS <| (compileExample ``ex₈ simpset (args := #[mkNatLit inputSize])).run' {} |>.run
+    let σ ← getAndResetDbgState
+    return (inputSize, res, σ)
+  for (n, (compiled, time), dbgState) in timings do
+    logInfo m!"ex₈[{n}] took {time}s"
+    logInfo m!"dbg: {repr dbgState}"
+
+    logInfo m!"{←ppMonad compiled}"
+    -- logInfo m!"res:\n{(←Sym.simp compiled (←compilerBindEqBind) |>.run).getResultExpr compiled}"
+
+  -- for n in inputSizes do
+  --   let (res, time) ← Dbg.timeS ∘ spoon <|
+  --     compileExample ``ex₈ (←(mapM_singlePass ∪ zeta ∪ monads ∪ explode ∪ bindMyAssoc_set))
+  --   timings := timings.push time
+  --   logInfo m!"res:\n{res}"
+  -- for timing in timings do
+
+set_option maxRecDepth 40000 in
+#eval bench
+
+-- 10 vec, [size 1409/272/272] of compiled
+opaque share : Nat → Option Nat
+
+def ex₉ {n : Nat} (vec : Vector Nat n) : Option Unit := do
+  let x ← (do let _ ← eq0 2; let x ← vec.mapM (fun x ↦ (share (x + 42) : Option _)); return x)
+  let _ ← x.mapM eq0
+
+set_option maxRecDepth 1024 in
+set_option trace.Clap.Compile.dbg true in
+set_option Clap.traversalDbg true in
+set_option trace.Clap.Compile false in
+#eval do
+  let (e, time) ← Dbg.timeS <| compileExample (args := #[toExpr 20]) ``ex₉
+    (←(SymSets.Vector.wrapped ∪
+      mapM_singlePass_pre ∪
+      getElem ∪
+      append ∪
+      explode -- ∪ zeta ∪ monads ∪ explode
+    ∪ compilerAssoc
+    -- ∪ bindMyAssoc_set
+    -- mapM_alt
+    )) |>.run' {} |>.run
+  logInfo m!"time: {time}"
+  -- let e' := Sym.simp e {}
+  let e' := Sym.simp e (←compilerBindEqBind)
+  let e' ← e'.run
+
+  logInfo m!"e: {e'.getResultExpr e}"
+  logInfo m!"{←(getAndResetDbgState <&> repr)}"
+
+set_option trace.Clap.Compile true in
+#eval spoon <| do
+  let e ← compileExampleJustSym ``ex₉
+    (←(mapM_alt ∪ zeta ∪ monads ∪ explode ∪ getElem ∪ append
+    -- ∪ compilerAssoc
+    ∪ bindMyAssoc_set
+    -- mapM_alt
+    ))
+  -- Pretty print (i.e. go back to `Bind.bind`)
+  return (←Sym.simp e (←compilerBindEqBind)).getResultExpr e
+
+-- set_option trace.Clap.Compile true in
+-- example {vec : Vector Nat 10} : ex₈ vec = .none := by
+--   unfold ex₈
+
+--   cbv
+--   -- compile_just_sym [SymSets.Vector.mapM]
+  -- rw [Option.bind_eq_bind]
+  -- rw [Option.bind_eq_bind]
+  -- -- rw [Option.bind_assoc]
+  -- compile_just_sym [compilerBindEqBind]
+  -- rw [bind_assoc]
+  -- rw [bind_assoc]
+  -- rw [bind_assoc]
+
+
+  -- compile_just_sym [compilerAssoc]
+  -- rw [bind_assoc]
+
+  -- #check bind_assoc
+-- set_option trace.Clap.Compile true in
+-- example {vec : Vector Nat 10} : ex₈' vec = sorry := by
+--   unfold ex₈'
+--   compile_just_sym [SymSets.Vector.foldlM, explode]
+--   rw [Option.bind_eq_bind]
+--   rw [Option.bind_eq_bind]
+--   compile_just_sym [compilerAssoc]
+--   compile_just_sym [compilerBindEqBind]
+
+-- def ex₈' (vec : Vector Nat 3) : Option Unit := do
+--   let x ← (do let _ )
+
+def ex₉ (vec : Vector Nat 160) : Option Unit := do
+  let res := (#v[0] ++ vec).extract 1 2
+  eq0 res[0]
+
+/--
+info: Compiled:
+fun vec => eq0 vec[0]
+-/
+#guard_msgs(info, whitespace := lax, drop warning) in
+#eval spoon <| do compileExampleJustSym ``ex₉ (←(extract ∪ append ∪ getElem ∪ zeta ∪ monads ∪ explode))
+
+def ex₁₀ (vec : Vector Nat 160) : Option Unit := do
+  let res := (#v[0] ++ vec).set 0 42
+  eq0 res[0]
+
+/--
+info: Compiled:
+fun vec => eq0 42
+-/
+#guard_msgs(info, whitespace := lax, drop warning) in
+#eval spoon <| do compileExampleJustSym ``ex₁₀ (←(set ∪ append ∪ getElem ∪ zeta ∪ monads ∪ explode))
+
+def ex₁₁ (vec : Vector Nat 160) : Option Unit := do
+  let res := vec.mapIdx fun i x ↦ x + i
+  eq0 res[0]
+
+/--
+info: Compiled:
+fun vec => eq0 (vec[0] + 0)
+-/
+#guard_msgs(info, whitespace := lax, drop warning) in
+#eval spoon <| do compileExampleJustSym ``ex₁₁ (←(mapIdx ∪ getElem ∪ zeta ∪ monads ∪ explode))
+
+-- def mixLast {t : ℕ} (state : Vector (F p) t) (M : Vector (Vector (F p) t) t) (s : ℕ) : F p :=
+--   (state.zipWith (fun (sj : F p) (row : Vector (F p) t) ↦ row[s]'sorry * sj) M).sum
+
+def ex₁₂ (vec : Vector Nat 4) : Option Unit := do
+  let state : Vector Nat 2 := #v[1, 2]
+  let M : Vector (Vector ℕ 2) 2 := #v[#v[1, 2], #v[3, 4]]
+  let res :=
+    (state.zipWith (fun (sj : ℕ) (row : Vector ℕ 2) ↦ row[0]'sorry * sj) M).sum
+  eq0 res
+
+/--
+info: Compiled:
+fun vec => eq0 7
+-/
+#guard_msgs(info, whitespace := lax, drop warning) in
+#eval spoon <| do compileExampleJustSym ``ex₁₂ (←(zeta ∪ monads ∪ explode ∪ zipWith ∪ sum ∪ getElem))
+def ex₁₃ (vec : Vector Nat 4) : Option Unit := do
+  let t := 2
+  let state : Vector Nat t := #v[1, 2]
+  let S : Vector Nat 6 := #v[3, 4, 5, 6, 7, 8]
+  let base : ℕ := (2 * 2 - 1) * 1
+  let s' : Vector _ t := ⟨S.extract base (base+t) |>.toArray, sorry⟩
+  let dotProduct := (state.zipWith (· * ·) s').sum
+  let tail := (state.drop 1).mapIdx (fun i sᵢ ↦ sᵢ + state[0]'sorry * S[base + t + i]'sorry)
+  let res : Vector Nat 2 := ⟨#[dotProduct] ++ tail.toArray, sorry⟩
+  eq0 res[0]
+
+/--
+info: Compiled:
+fun vec => eq0 20
+-/
+#guard_msgs(info, whitespace := lax, drop warning) in
+#eval spoon <| do
+  compileExampleJustSym ``ex₁₃
+    (←(zeta ∪ monads ∪ explode ∪ zipWith ∪ sum ∪ extract ∪ toArray ∪ mapIdx ∪ append ∪ getElem ∪ drop ∪ extract))
+
+opaque p : Nat
+opaque q : Nat
+axiom a : p = q
+def test := fun x : Nat => (x,x,x,x,x,x,x,x,x,x,x,x,x,x,x,x,x,x,x,x)
+set_option pp.exprSizes true in
+set_option maxRecDepth 1000 in
+example : (fun x : Nat => (x,x,x,x,x,x,x,x,x,x,x,x,x,x,x,x,x,x,x,x)) p = sorry := by
+  sym_simp [beta]
+
+opaque f : (Nat → Nat) → Nat
+def exp := fun x : Nat ↦ f (fun x : Nat ↦ f (fun _ : Nat ↦ 0))
+
+def abc : Sym.SymM Unit := do
+  let expr := (←getEnv).find? ``Clap.Compiler.ExampruSym.exp |>.get!.value!
+  let s := (← get).share.set.toList
+  logInfo m!"{s.map (·.expr)}"
+  let e ← Sym.shareCommon expr
+  let s := (← get).share.set.toList
+  logInfo m!"{s.map (·.expr)}"
+
+#eval abc.run
+
+end ExampruSym
