Clap/Test/Compiler/Traverse/Prelude.lean
@@ -1,0 +1,83 @@
+import Clap.Compiler.Traverse
+
+namespace ExampruSym
+
+open Clap.Compiler
+
+opaque F : ℕ → Option ℕ
+opaque G : ℕ → Option ℕ
+opaque H : ℕ → Option ℕ
+
+def testSymSet :=
+  -- ExampruSym.NewTraversal.Dom.flattenBinds_pre
+  -- SymSets.Vector.unwrap_s
+  -- ExampruSym.NewTraversal.Dom.flattenBindsAny_pre
+  -- ∪ ExampruSym.NewTraversal.Dom.bindPureMany_pre
+  -- ∪ Clap.Compiler.ExampruSym.NewTraversal.Dom.strategiaMagna
+  -- ∪
+  SymSets.General.optionPureApply
+  -- ∪ SymSets.Vector.foldlM_stagger_post
+  ∪ SymSets.Vector.unfold_generic_collection_functions_pre
+  -- ∪ SymSets.Vector.foldlM_post
+  ∪ SymSets.General.beta
+  ∪ SymSets.General.zeta
+  ∪ SymSets.List.range
+  ∪ Clap.SymSets.General.ground
+
+open Lean in
+def runTest (uncompiledExpr : Expr) (eval : Bool := true)
+            (isUsingTopLevelStrategy : Bool := false) := spoon <| do
+  let uncompiledTypeExpr ← Meta.inferType uncompiledExpr
+  let expectedType := (Option ℕ)
+
+  let time ← IO.monoMsNow
+  logInfo m!"Compiling {uncompiledExpr}"
+  let compiled ←
+    if isUsingTopLevelStrategy
+    then ExampruSym.NewTraversal.Dom.compilaCumStrategiaMagna uncompiledExpr (←testSymSet)
+    else compileJustSym uncompiledExpr (←testSymSet)
+  Clap.Dbg.timeSince time "Compilation took:"
+  logInfo m!"Compiled to {compiled}"
+
+  if !eval then return compiled
+
+  let dbgState ← getAndResetDbgState
+  logInfo m!"{←dbgState.pretty}"
+  -- Pretty print (i.e. go back to `Bind.bind`)
+  let formatted := (
+    ←Lean.Meta.Sym.simp compiled (←SymSets.General.compilerBindEqBind)
+  ).getResultExpr compiled
+  let defEq ← Lean.Meta.isDefEq uncompiledExpr compiled
+  if defEq then
+    Lean.logInfo m!"Compiled expression defEq"
+  else
+    Lean.logInfo m!"Compiled expression not defEq"
+
+  let uncompiledEvaluated ← Lean.Core.tryCatchRuntimeEx
+    do
+      let uncompiledEvaluated ← (unsafe Lean.Meta.evalExpr expectedType uncompiledTypeExpr uncompiledExpr).run
+      return uncompiledEvaluated.1
+    fun exception => do
+      Lean.logInfo m!"Failed to evaluate uncompiled test expression with given type"
+      throwError m!"{exception.toMessageData}"
+
+  let compiledEvaluated ← Lean.Core.tryCatchRuntimeEx
+    do
+      let compiledEvaluated ← (unsafe Lean.Meta.evalExpr expectedType uncompiledTypeExpr compiled).run
+      return compiledEvaluated.1
+    fun exception => do
+      Lean.logInfo m!"Failed to evaluate compiled test expression with given type"
+      throwError m!"{exception.toMessageData}"
+
+  if uncompiledEvaluated == compiledEvaluated then
+    Lean.logInfo m!"Compiled expression evalutes equal: {uncompiledEvaluated} == {compiledEvaluated}"
+  else
+    Lean.logError m!"Compiled expression evaluates unequal\nUncompiled: {uncompiledEvaluated} ≠ Compiled: {compiledEvaluated}"
+  return formatted
+
+open Lean in
+def runTestByName (testName : Name) (eval : Bool := true) (isUsingTopLevelStrategy : Bool := false) : MetaM Unit := do
+  let .some constantInfo := (←getEnv).find? testName | throwError m!"Undeclared constant:\n{testName}"
+  runTest constantInfo.value! eval isUsingTopLevelStrategy
+
+end ExampruSym
