Clap/Test/Compiler/Traverse/Reduction.lean
@@ -1,0 +1,27 @@
+import Clap.Test.Compiler.Traverse.Prelude
+
+namespace ExampruSym
+
+namespace NewTraversal
+
+open Clap.Compiler
+
+def testBetaReductionOneArg : Option ℕ := do
+  let a ← ((λ x: ℕ => (.some x)) 5)
+  return a
+
+def testBetaReductionTwoArgs : Option ℕ := do
+  let a ← (λ x y => .some (x - y)) 1 2
+  return a
+
+
+-- set_option trace.Clap.Compile true in
+-- set_option Clap.traversalDbg true in
+-- set_option trace.Clap.Compile.dbg true in
+-- set_option maxRecDepth 100000 in
+#eval runTestByName ``testBetaReductionOneArg
+#eval runTestByName ``testBetaReductionTwoArgs
+
+end NewTraversal
+
+end ExampruSym
